Subtraction_Hoare.thy
@@ -8,31 +8,31 @@
  *  Author: Albert Rizaldi, NTU Singapore
  *)
 
-theory Addition_Hoare
+theory Subtraction_Hoare
   imports VHDL_Hoare_Complete Bits_Int_Aux
 begin
 
 datatype sig = A | B | C
 
-definition add :: "sig conc_stmt" where
-  "add \<equiv> process {A, B} : Bassign_trans C (Badd (Bsig A) (Bsig B)) 1"
+definition sub :: "sig conc_stmt" where
+  "sub \<equiv> process {A, B} : Bassign_trans C (Bsub (Bsig A) (Bsig B)) 1"
 
 lemma potential_tyenv:
-  assumes "seq_wt \<Gamma> (Bassign_trans C (Badd (Bsig A) (Bsig B)) 1)"
+  assumes "seq_wt \<Gamma> (Bassign_trans C (Bsub (Bsig A) (Bsig B)) 1)"
   shows "\<exists>len1>0. \<exists>len2>0. \<Gamma> A = Lty Uns len1 \<and> \<Gamma> B = Lty Uns len2 \<and> \<Gamma> C = Lty Uns (max len1 len2)
-                         \<or> \<Gamma> A = Lty Sig len1 \<and> \<Gamma> B = Lty Sig len2 \<and> \<Gamma> C = Lty Sig (max len1 len2)"
+                   \<or> \<Gamma> A = Lty Sig len1 \<and> \<Gamma> B = Lty Sig len2 \<and> \<Gamma> C = Lty Sig (max len1 len2)"
 proof (rule seq_wt_cases(4)[OF assms])
-  assume "bexp_wt \<Gamma> (Badd (Bsig A) (Bsig B)) (\<Gamma> C)"
+  assume "bexp_wt \<Gamma> (Bsub (Bsig A) (Bsig B)) (\<Gamma> C)"
   obtain len1 len2 where " \<Gamma> A = Lty Uns len1 \<and> \<Gamma> B = Lty Uns len2 \<and> \<Gamma> C = Lty Uns (max len1 len2)
                               \<or> \<Gamma> A = Lty Sig len1 \<and> \<Gamma> B = Lty Sig len2 \<and> \<Gamma> C = Lty Sig (max len1 len2)"
-          and "0 < len1" and "0 < len2"
-    by (rule bexp_wt_cases(11)[OF \<open>bexp_wt \<Gamma> (Badd (Bsig A) (Bsig B)) (\<Gamma> C)\<close>])
+      and "0 < len1" and "0 < len2"
+    by (rule bexp_wt_cases(13)[OF \<open>bexp_wt \<Gamma> (Bsub (Bsig A) (Bsig B)) (\<Gamma> C)\<close>])
        (metis bexp_wt_cases(9))+
   thus ?thesis
     by auto
 qed
 
-locale unsigned_addition =
+locale unsigned_subition =
   fixes \<Gamma> :: "sig tyenv"
   fixes len len1 len2 :: nat
   assumes len_def: "len = max len1 len2"
@@ -41,18 +41,13 @@ locale unsigned_addition =
 begin
 
 lemma well_typed:
-  "seq_wt \<Gamma> (Bassign_trans C (Badd (Bsig A) (Bsig B)) 1)"
+  "seq_wt \<Gamma> (Bassign_trans C (Bsub (Bsig A) (Bsig B)) 1)"
   apply (rule seq_wt.intros(4))
-  unfolding ctype len_def apply (rule bexp_wt.intros(15))
-  unfolding atype[THEN sym] btype[THEN sym] 
-     apply (rule bexp_wt.intros(3))+
-   apply (rule len1)
-  apply (rule len2)
-  done
+  unfolding ctype len_def apply (rule bexp_wt.intros(19))
+  unfolding atype[THEN sym] btype[THEN sym]  apply (rule bexp_wt.intros(3))+
+  using len1 len2 by auto
 
 abbreviation "lof_wline tw sig n \<equiv> lval_of (wline_of tw sig n)"
-
-term "bin_to_bl len (bl_to_bin bs1 + bl_to_bin bs2)"
 
 text \<open>Here we factor out common expression in both inv1 and inv2. It is parametrised by the index
 we are interested with for C (first argument) and A (the second argument). Note that the index
@@ -61,7 +56,7 @@ we are interested with for A should be the same as the index for B.\<close>
 definition property :: "nat \<Rightarrow> nat \<Rightarrow> sig assn2" where
   "property idxc idx =
       (\<lambda>tw. lof_wline tw C idxc =
-                  bin_to_bl len (bl_to_bin (lof_wline tw A idx) + bl_to_bin (lof_wline tw B idx)))"
+                  bin_to_bl len (bl_to_bin (lof_wline tw A idx) - bl_to_bin (lof_wline tw B idx)))"
 
 definition inv :: "sig assn2" where
   "inv tw \<equiv> (\<forall>i < fst tw. property (i + 1) i tw)"
@@ -73,7 +68,7 @@ abbreviation "next_world tw \<equiv> (next_time_world tw, snd tw)"
 
 lemma inv_next_time:
   assumes "inv tw"
-  assumes "beval_world_raw2 tw (Badd (Bsig A) (Bsig B)) v" and "type_of v = Lty Uns len"
+  assumes "beval_world_raw2 tw (Bsub (Bsig A) (Bsig B)) v" and "type_of v = Lty Uns len"
   defines "tw' \<equiv> tw[C, 1 :=\<^sub>2 v]"
   shows   "inv (next_time_world tw', snd tw')"
   unfolding inv_def
@@ -94,9 +89,9 @@ proof (rule, rule)
   { assume "i < fst tw"
     have "lof_wline tw' C (i + 1) = lof_wline tw C (i + 1)"
       by (metis \<open>i < get_time tw\<close> add_mono1 tw'_def worldline_upd2_before_dly)
-    also have "... = bin_to_bl len (bl_to_bin (lof_wline tw A i) + bl_to_bin (lof_wline tw B i))"
+    also have "... = bin_to_bl len (bl_to_bin (lof_wline tw A i) - bl_to_bin (lof_wline tw B i))"
       using assms(1) \<open>i < fst tw\<close> unfolding inv_def property_def by auto
-    also have "... = bin_to_bl len (bl_to_bin (lof_wline tw' A i) + bl_to_bin (lof_wline tw' B i))"
+    also have "... = bin_to_bl len (bl_to_bin (lof_wline tw' A i) - bl_to_bin (lof_wline tw' B i))"
       by (metis \<open>i < get_time tw\<close> add.commute trans_less_add2 tw'_def worldline_upd2_before_dly)
     finally have "property (i + 1) i (next_time_world tw', snd tw')"
       unfolding property_def by auto }
@@ -114,17 +109,17 @@ proof (rule, rule)
       less_add_one tw'_def worldline_upd2_before_dly)+
     moreover have "property (fst tw + 1) (fst tw) tw'"
     proof -
-      have assm2: "beval_world_raw (snd tw) (fst tw) (Badd (Bsig A) (Bsig B)) v"
+      have assm2: "beval_world_raw (snd tw) (fst tw) (Bsub (Bsig A) (Bsig B)) v"
         using assms(2) unfolding beval_world_raw2_def by auto
       have "wline_of tw' C (fst tw + 1) = v"
         unfolding tw'_def worldline_upd2_def worldline_upd_def by auto
-      also have "... =  Lv Uns (bin_to_bl_aux len (bl_to_bin (lof_wline tw A (fst tw)) + bl_to_bin (lof_wline tw B (fst tw))) [])"
+      also have "... =  Lv Uns (bin_to_bl_aux len (bl_to_bin (lof_wline tw A (fst tw)) - bl_to_bin (lof_wline tw B (fst tw))) [])"
         apply (rule beval_world_raw_cases[OF assm2])
         apply ( erule beval_cases)+
         unfolding state_of_world_def using atype btype
         apply (metis assms(3) bin_to_bl_def comp_def size_bin_to_bl ty.inject type_of.simps(2) val.sel(3))
         using assms(3) by auto
-      also have "... =  Lv Uns (bin_to_bl_aux len (bl_to_bin (lof_wline tw' A (fst tw)) + bl_to_bin (lof_wline tw' B (fst tw))) [])"
+      also have "... =  Lv Uns (bin_to_bl_aux len (bl_to_bin (lof_wline tw' A (fst tw)) - bl_to_bin (lof_wline tw' B (fst tw))) [])"
         by (metis Suc_eq_plus1 \<open>lval_of (wline_of tw' A i) = lval_of (wline_of tw' A (get_time tw))\<close>
         \<open>lval_of (wline_of tw' B i) = lval_of (wline_of tw' B (get_time tw))\<close> lessI tw'_def
         worldline_upd2_before_dly)
@@ -144,17 +139,17 @@ proof (rule, rule)
       by auto
     moreover have "property (fst tw + 1) (fst tw) tw'"
     proof -
-      have assm2: "beval_world_raw (snd tw) (fst tw) (Badd (Bsig A) (Bsig B)) v"
+      have assm2: "beval_world_raw (snd tw) (fst tw) (Bsub (Bsig A) (Bsig B)) v"
         using assms(2) unfolding beval_world_raw2_def by auto
       have "wline_of tw' C (fst tw + 1) = v"
         unfolding tw'_def worldline_upd2_def worldline_upd_def by auto
-      also have "... =  Lv Uns (bin_to_bl_aux len (bl_to_bin (lof_wline tw A (fst tw)) + bl_to_bin (lof_wline tw B (fst tw))) [])"
+      also have "... =  Lv Uns (bin_to_bl_aux len (bl_to_bin (lof_wline tw A (fst tw)) - bl_to_bin (lof_wline tw B (fst tw))) [])"
         apply (rule beval_world_raw_cases[OF assm2])
         apply ( erule beval_cases)+
         unfolding state_of_world_def using atype btype
         apply (metis assms(3) bin_to_bl_def comp_def size_bin_to_bl ty.inject type_of.simps(2) val.sel(3))
         using assms(3) by auto
-      also have "... =  Lv Uns (bin_to_bl_aux len (bl_to_bin (lof_wline tw' A (fst tw)) + bl_to_bin (lof_wline tw' B (fst tw))) [])"
+      also have "... =  Lv Uns (bin_to_bl_aux len (bl_to_bin (lof_wline tw' A (fst tw)) - bl_to_bin (lof_wline tw' B (fst tw))) [])"
         by (metis less_add_one tw'_def worldline_upd2_before_dly)
       finally show ?thesis
         unfolding property_def bin_to_bl_def by auto
@@ -171,40 +166,39 @@ qed
 
 lemma type_correctness_length:
   assumes "wityping \<Gamma> (snd tw)"
-  assumes "beval_world_raw2 tw (Badd (Bsig A) (Bsig B)) v"
+  assumes "beval_world_raw2 tw (Bsub (Bsig A) (Bsig B)) v"
   shows   "type_of v = Lty Uns len"
 proof -
-  have "beval_world_raw (snd tw) (fst tw) (Badd (Bsig A) (Bsig B)) v"
+  have "beval_world_raw (snd tw) (fst tw) (Bsub (Bsig A) (Bsig B)) v"
     using assms(2) unfolding beval_world_raw2_def by auto
   have "type_of (state_of_world (snd tw) (fst tw) A) = Lty Uns len1" and
        "type_of (state_of_world (snd tw) (fst tw) B) = Lty Uns len2"
     using assms(1) unfolding wityping_def
     by (simp add: atype btype state_of_world_def wtyping_def)+
   show ?thesis
-    apply (rule beval_world_raw_cases[OF \<open>beval_world_raw (snd tw) (fst tw) (Badd (Bsig A) (Bsig B)) v\<close>])
+    apply (rule beval_world_raw_cases[OF \<open>beval_world_raw (snd tw) (fst tw) (Bsub (Bsig A) (Bsig B)) v\<close>])
     apply (erule beval_cases)
     apply (metis (no_types, lifting) \<open>type_of (state_of_world (snd tw) (get_time tw) A) = Lty Uns len1\<close> \<open>type_of (state_of_world (snd tw) (get_time tw) B) = Lty Uns len2\<close> add.right_neutral beval_cases(1) len_def list.size(3) size_bin_to_bl_aux ty.inject type_of.simps(2))
-    apply (metis (no_types, lifting) \<open>type_of (state_of_world (snd tw) (get_time tw) A) = Lty Uns len1\<close> beval_cases(1) signedness.distinct(5) ty.inject type_of.simps(2))
-    done
+    by  (metis (no_types, hide_lams) \<open>type_of (state_of_world (snd tw) (get_time tw) A) = Lty Uns len1\<close> beval_cases(1) signedness.distinct(5) ty.inject type_of.simps(2))
 qed
 
-lemma add_seq_hoare_next_time:
+lemma sub_seq_hoare_next_time:
   "\<turnstile> [\<lambda>tw. inv tw \<and> wityping \<Gamma> (snd tw)]
-        Bassign_trans C (Badd (Bsig A) (Bsig B)) 1
+        Bassign_trans C (Bsub (Bsig A) (Bsig B)) 1
      [\<lambda>tw. inv (next_world tw)]"
   apply (rule Conseq2[where Q="\<lambda>tw. inv (next_world tw) \<and> wityping \<Gamma> (snd tw)", rotated 1], rule Assign2, simp)
   using inv_next_time type_correctness_length
   by (metis ctype snd_conv worldline_upd2_def worldline_upd_preserve_wityping)
 
-lemma add_seq_hoare_next_time0:
+lemma sub_seq_hoare_next_time0:
   "\<turnstile> [\<lambda>tw. fst tw = 0 \<and> wityping \<Gamma> (snd tw)]
-        Bassign_trans C (Badd (Bsig A) (Bsig B)) 1
+        Bassign_trans C (Bsub (Bsig A) (Bsig B)) 1
      [\<lambda>tw. inv (next_world tw)]"
   apply (rule Conseq2[where Q="\<lambda>tw. inv (next_world tw) \<and> wityping \<Gamma> (snd tw)", rotated 1], rule Assign2, simp)
   using inv_next_time type_correctness_length unfolding inv_def
   by (metis ctype gr_implies_not0 snd_conv worldline_upd2_def worldline_upd_preserve_wityping)
 
-lemma add_conc_hoare:
+lemma sub_conc_hoare:
   "\<And>tw. inv tw \<and> inv2 tw \<and> disjnt {A, B} (event_of tw) \<Longrightarrow> inv (next_world tw)"
 proof -
   fix tw
@@ -241,7 +235,7 @@ proof -
     unfolding inv_def by auto
 qed
 
-lemma add_conc_hoare2:
+lemma sub_conc_hoare2:
   "\<And>tw. inv tw \<and> inv2 tw \<and> disjnt {A, B} (event_of tw) \<Longrightarrow> inv2 (next_world tw)"
 proof -
   fix tw
@@ -273,7 +267,7 @@ qed
 
 lemma inv2_next_time:
   fixes tw
-  assumes "beval_world_raw2 tw (Badd (Bsig A) (Bsig B)) v" and "type_of v = Lty Uns len"
+  assumes "beval_world_raw2 tw (Bsub (Bsig A) (Bsig B)) v" and "type_of v = Lty Uns len"
   defines "tw' \<equiv> tw[C, 1 :=\<^sub>2 v]"
   shows   "inv2 (next_time_world tw', snd tw')"
   unfolding inv2_def
@@ -324,7 +318,7 @@ proof (rule, rule, rule)
     finally show "wline_of (next_world tw') B ?t' = wline_of tw B (fst tw)"
       by auto
   qed
-  have assm2: "beval_world_raw (snd tw) (fst tw) (Badd (Bsig A) (Bsig B)) v"
+  have assm2: "beval_world_raw (snd tw) (fst tw) (Bsub (Bsig A) (Bsig B)) v"
     using assms(1) unfolding beval_world_raw2_def by auto
   have "wline_of (next_world tw') C (i + 1) = v"
   proof -
@@ -334,7 +328,7 @@ proof (rule, rule, rule)
     thus ?thesis
       by auto
   qed
-  also have "lval_of ... = bin_to_bl len (bl_to_bin (lof_wline tw A (fst tw)) + bl_to_bin (lof_wline tw B (fst tw)))"
+  also have "lval_of ... = bin_to_bl len (bl_to_bin (lof_wline tw A (fst tw)) - bl_to_bin (lof_wline tw B (fst tw)))"
     apply (rule beval_world_raw_cases[OF assm2])
     apply (erule beval_cases)+
     apply (metis assms(2) beval_raw.intros(1) beval_world_raw.simps beval_world_raw2_Bsig beval_world_raw2_def beval_world_raw_deterministic bin_to_bl_def size_bin_to_bl ty.inject type_of.simps(2) val.sel(3))
@@ -345,130 +339,130 @@ proof (rule, rule, rule)
     by auto
 qed
 
-lemma add_seq_hoare_next_time1:
-  shows "\<turnstile> [\<lambda>tw. wityping \<Gamma> (snd tw)] Bassign_trans C (Badd (Bsig A) (Bsig B)) 1 [\<lambda>tw. inv2 (next_time_world tw, snd tw)]"
+lemma sub_seq_hoare_next_time1:
+  shows "\<turnstile> [\<lambda>tw. wityping \<Gamma> (snd tw)] Bassign_trans C (Bsub (Bsig A) (Bsig B)) 1 [\<lambda>tw. inv2 (next_time_world tw, snd tw)]"
   apply (rule Assign2_altI)
   using inv2_next_time type_correctness_length by blast
 
-lemma add_conc_hoare3:
-  "\<turnstile> \<lbrace>\<lambda>tw. (inv tw \<and> wityping \<Gamma> (snd tw)) \<and> inv2 tw\<rbrace> add \<lbrace>\<lambda>tw. inv (next_time_world tw, snd tw) \<and> inv2 (next_time_world tw, snd tw)\<rbrace>"
-  unfolding add_def
+lemma sub_conc_hoare3:
+  "\<turnstile> \<lbrace>\<lambda>tw. (inv tw \<and> wityping \<Gamma> (snd tw)) \<and> inv2 tw\<rbrace> sub \<lbrace>\<lambda>tw. inv (next_time_world tw, snd tw) \<and> inv2 (next_time_world tw, snd tw)\<rbrace>"
+  unfolding sub_def
   apply (rule Single)
    apply (rule Conj)
     apply (rule strengthen_precondition)
   apply (rule strengthen_precondition)
-    apply (rule add_seq_hoare_next_time)
+    apply (rule sub_seq_hoare_next_time)
   apply (rule strengthen_precondition)
    apply (rule strengthen_precondition)
    apply (rule strengthen_precondition2)
-   apply (rule add_seq_hoare_next_time1)
-  using add_conc_hoare add_conc_hoare2 by blast
+   apply (rule sub_seq_hoare_next_time1)
+  using sub_conc_hoare sub_conc_hoare2 by blast
 
-lemma seq_wt_add:
-  "seq_wt \<Gamma> (Bassign_trans C (Badd (Bsig A) (Bsig B)) 1)"
+lemma seq_wt_sub:
+  "seq_wt \<Gamma> (Bassign_trans C (Bsub (Bsig A) (Bsig B)) 1)"
   using well_typed by blast
 
-lemma add_conc_hoare4:
-  "\<turnstile> \<lbrace>\<lambda>tw. (inv tw \<and> wityping \<Gamma> (snd tw)) \<and> inv2 tw\<rbrace> add \<lbrace>\<lambda>tw. (inv (next_time_world tw, snd tw) \<and> wityping \<Gamma> (snd tw)) \<and> inv2 (next_time_world tw, snd tw)\<rbrace>"
+lemma sub_conc_hoare4:
+  "\<turnstile> \<lbrace>\<lambda>tw. (inv tw \<and> wityping \<Gamma> (snd tw)) \<and> inv2 tw\<rbrace> sub \<lbrace>\<lambda>tw. (inv (next_time_world tw, snd tw) \<and> wityping \<Gamma> (snd tw)) \<and> inv2 (next_time_world tw, snd tw)\<rbrace>"
   apply (rule Conj2)
    apply (rule Conj2)
-    apply (rule weaken_post_conc_hoare[OF _ add_conc_hoare3], blast)
+    apply (rule weaken_post_conc_hoare[OF _ sub_conc_hoare3], blast)
    apply (rule strengthen_pre_conc_hoare[rotated])
-    apply (unfold add_def, rule single_conc_stmt_preserve_wityping_hoare)
-    apply (rule seq_wt_add)
+    apply (unfold sub_def, rule single_conc_stmt_preserve_wityping_hoare)
+    apply (rule seq_wt_sub)
    apply blast
-  apply (fold add_def, rule weaken_post_conc_hoare[OF _ add_conc_hoare3], blast)
+  apply (fold sub_def, rule weaken_post_conc_hoare[OF _ sub_conc_hoare3], blast)
   done
 
-lemma add_conc_sim':
-  "\<turnstile>\<^sub>s \<lbrace>\<lambda>tw. (inv tw \<and> wityping \<Gamma> (snd tw)) \<and> inv2 tw\<rbrace> add \<lbrace>\<lambda>tw. (inv tw \<and> wityping \<Gamma> (snd tw)) \<and> inv2 tw\<rbrace>"
+lemma sub_conc_sim':
+  "\<turnstile>\<^sub>s \<lbrace>\<lambda>tw. (inv tw \<and> wityping \<Gamma> (snd tw)) \<and> inv2 tw\<rbrace> sub \<lbrace>\<lambda>tw. (inv tw \<and> wityping \<Gamma> (snd tw)) \<and> inv2 tw\<rbrace>"
   apply (rule While)
-  apply (unfold snd_conv, rule add_conc_hoare4)
+  apply (unfold snd_conv, rule sub_conc_hoare4)
   done
 
-lemma add_conc_sim2:
-  "\<turnstile>\<^sub>s \<lbrace>\<lambda>tw. (inv tw \<and> wityping \<Gamma> (snd tw)) \<and> inv2 tw\<rbrace> add \<lbrace>inv\<rbrace>"
-  using add_conc_sim' Conseq_sim by blast
+lemma sub_conc_sim2:
+  "\<turnstile>\<^sub>s \<lbrace>\<lambda>tw. (inv tw \<and> wityping \<Gamma> (snd tw)) \<and> inv2 tw\<rbrace> sub \<lbrace>inv\<rbrace>"
+  using sub_conc_sim' Conseq_sim by blast
 
-lemma init_sat_add_inv:
-  "init_sim_hoare (\<lambda>tw. fst tw = 0 \<and> wityping \<Gamma> (snd tw)) add (\<lambda>tw. inv tw \<and> wityping \<Gamma> (snd tw))"
-  unfolding add_def
+lemma init_sat_sub_inv:
+  "init_sim_hoare (\<lambda>tw. fst tw = 0 \<and> wityping \<Gamma> (snd tw)) sub (\<lambda>tw. inv tw \<and> wityping \<Gamma> (snd tw))"
+  unfolding sub_def
   apply (rule AssignI)
   apply (rule SingleI)
   apply (rule Conj)
-  unfolding snd_conv apply(rule add_seq_hoare_next_time0)
+  unfolding snd_conv apply(rule sub_seq_hoare_next_time0)
   apply (rule strengthen_precondition2)
   by (metis seq_stmt_preserve_wityping_hoare well_typed)
 
-lemma init_sat_add_inv2:
-  "init_sim_hoare (\<lambda>tw. wityping \<Gamma> (snd tw)) add inv2"
-  unfolding add_def
+lemma init_sat_sub_inv2:
+  "init_sim_hoare (\<lambda>tw. wityping \<Gamma> (snd tw)) sub inv2"
+  unfolding sub_def
   apply (rule AssignI)
   apply (rule SingleI)
-  unfolding snd_conv apply (rule add_seq_hoare_next_time1)
+  unfolding snd_conv apply (rule sub_seq_hoare_next_time1)
   done
 
-lemma init_sat_add_inv_comb:
-  shows "init_sim_hoare (\<lambda>tw. fst tw = 0 \<and> wityping \<Gamma> (snd tw)) add  (\<lambda>tw. (inv tw \<and> wityping \<Gamma> (snd tw)) \<and> inv2 tw)"
+lemma init_sat_sub_inv_comb:
+  shows "init_sim_hoare (\<lambda>tw. fst tw = 0 \<and> wityping \<Gamma> (snd tw)) sub  (\<lambda>tw. (inv tw \<and> wityping \<Gamma> (snd tw)) \<and> inv2 tw)"
   apply (rule ConjI_sim)
-  apply (rule init_sat_add_inv)
+  apply (rule init_sat_sub_inv)
   apply (rule ConseqI_sim[rotated])
-  apply (rule init_sat_add_inv2)
+  apply (rule init_sat_sub_inv2)
   by blast+
 
-lemma add_correctness:
-  assumes "sim_fin w (i + 1) add tw'" and "wityping \<Gamma> w"
+lemma sub_correctness:
+  assumes "sim_fin w (i + 1) sub tw'" and "wityping \<Gamma> w"
   shows   "property (i + 1) i tw'"
 proof -
-  obtain tw where "init_sim (0, w) add tw" and  "tw, i + 1, add \<Rightarrow>\<^sub>S tw'"
+  obtain tw where "init_sim (0, w) sub tw" and  "tw, i + 1, sub \<Rightarrow>\<^sub>S tw'"
     using premises_sim_fin_obt[OF assms(1)] by auto
   hence "i + 1 < fst tw'"
     using world_maxtime_lt_fst_tres  by blast
-  have "conc_stmt_wf add"
-    unfolding conc_stmt_wf_def add_def by auto
-  moreover have "nonneg_delay_conc add"
-    unfolding add_def by auto
-  ultimately have "init_sim_valid (\<lambda>tw. fst tw = 0 \<and> wityping \<Gamma> (snd tw)) add (\<lambda>tw. (inv tw \<and> wityping \<Gamma> (snd tw)) \<and> inv2 tw)"
-    using init_sim_hoare_soundness[OF init_sat_add_inv_comb]
-    by (metis (no_types, lifting) conc_wt_cases(1) init_sat_add_inv_comb
-    init_sim_hoare_soundness add_def strengthen_precondition_init_sim_hoare)
+  have "conc_stmt_wf sub"
+    unfolding conc_stmt_wf_def sub_def by auto
+  moreover have "nonneg_delay_conc sub"
+    unfolding sub_def by auto
+  ultimately have "init_sim_valid (\<lambda>tw. fst tw = 0 \<and> wityping \<Gamma> (snd tw)) sub (\<lambda>tw. (inv tw \<and> wityping \<Gamma> (snd tw)) \<and> inv2 tw)"
+    using init_sim_hoare_soundness[OF init_sat_sub_inv_comb]
+    by (metis (no_types, lifting) conc_wt_cases(1) init_sat_sub_inv_comb
+    init_sim_hoare_soundness sub_def strengthen_precondition_init_sim_hoare)
   hence "inv tw \<and> wityping \<Gamma> (snd tw) \<and> inv2 tw"
-    using \<open>init_sim (0, w) add tw\<close> fst_conv assms(2) unfolding init_sim_valid_def
+    using \<open>init_sim (0, w) sub tw\<close> fst_conv assms(2) unfolding init_sim_valid_def
     by (metis snd_conv)
   hence "inv tw" and "inv2 tw" and "wityping \<Gamma> (snd tw)"
     by auto
-  moreover have "\<Turnstile>\<^sub>s \<lbrace>\<lambda>tw. (inv tw \<and> wityping \<Gamma> (snd tw)) \<and> inv2 tw\<rbrace> add \<lbrace>inv\<rbrace>"
-    using conc_sim_soundness[OF add_conc_sim2] \<open>conc_stmt_wf add\<close> \<open>nonneg_delay_conc add\<close>
+  moreover have "\<Turnstile>\<^sub>s \<lbrace>\<lambda>tw. (inv tw \<and> wityping \<Gamma> (snd tw)) \<and> inv2 tw\<rbrace> sub \<lbrace>inv\<rbrace>"
+    using conc_sim_soundness[OF sub_conc_sim2] \<open>conc_stmt_wf sub\<close> \<open>nonneg_delay_conc sub\<close>
     by auto
   ultimately have "inv tw'"
-    using \<open>tw, i + 1, add \<Rightarrow>\<^sub>S tw'\<close> unfolding sim_hoare_valid_def by blast
+    using \<open>tw, i + 1, sub \<Rightarrow>\<^sub>S tw'\<close> unfolding sim_hoare_valid_def by blast
   with \<open>i + 1 < fst tw'\<close> show ?thesis
     unfolding inv_def by auto
 qed
 
-corollary add_correctness2:
-  assumes "sim_fin w (i + 1) add tw'" and "wityping \<Gamma> w"
+corollary sub_correctness2:
+  assumes "sim_fin w (i + 1) sub tw'" and "wityping \<Gamma> w"
   defines "bsA \<equiv> lof_wline tw' A i"
   defines "bsB \<equiv> lof_wline tw' B i"
   defines "bsC \<equiv> lof_wline tw' C (i + 1)"
   shows   "(\<Sum>i = 0..<length bsC. (int \<circ> of_bool) (rev bsC ! i) * 2 ^ i) =
-          ((\<Sum>i = 0..<length bsA. (int \<circ> of_bool) (rev bsA ! i) * 2 ^ i) +
+          ((\<Sum>i = 0..<length bsA. (int \<circ> of_bool) (rev bsA ! i) * 2 ^ i) -
            (\<Sum>i = 0..<length bsB. (int \<circ> of_bool) (rev bsB ! i) * 2 ^ i) ) mod 2 ^ len "
 proof -
   have "property (i + 1) i tw'"
-    using add_correctness[OF assms(1-2)] by auto
+    using sub_correctness[OF assms(1-2)] by auto
   hence "lof_wline tw' C (i + 1) =
-                  bin_to_bl len (bl_to_bin (lof_wline tw' A i) + bl_to_bin (lof_wline tw' B i))"
+                  bin_to_bl len (bl_to_bin (lof_wline tw' A i) - bl_to_bin (lof_wline tw' B i))"
     unfolding property_def by auto
-  hence "bsC = bin_to_bl len (bl_to_bin bsA + bl_to_bin bsB)" (is "_ = ?rhs")
+  hence "bsC = bin_to_bl len (bl_to_bin bsA - bl_to_bin bsB)" (is "_ = ?rhs")
     unfolding bsA_def bsB_def bsC_def by auto
   hence "bl_to_bin bsC = bl_to_bin ?rhs"
     by auto
-  also have "... = bintrunc len (bl_to_bin bsA + bl_to_bin bsB)"
+  also have "... = bintrunc len (bl_to_bin bsA - bl_to_bin bsB)"
     unfolding bin_bl_bin by auto
-  also have "... = (bl_to_bin bsA + bl_to_bin bsB) mod 2 ^ len"
+  also have "... = (bl_to_bin bsA - bl_to_bin bsB) mod 2 ^ len"
     unfolding bintrunc_mod2p by auto
-  finally have "bl_to_bin bsC = (bl_to_bin bsA + bl_to_bin bsB) mod 2 ^ len"
+  finally have "bl_to_bin bsC = (bl_to_bin bsA - bl_to_bin bsB) mod 2 ^ len"
     by auto
   thus ?thesis
     unfolding bl_to_bin_correctness by auto
@@ -481,14 +475,13 @@ locale signed_addition =
   fixes len len1 len2 :: nat
   assumes len_def: "len = max len1 len2"
   assumes atype: "\<Gamma> A = Lty Sig len1" and btype: "\<Gamma> B = Lty Sig len2" and ctype: "\<Gamma> C = Lty Sig len"
-  assumes len1 : "0 < len1" and len2: "0 < len2"
+  assumes len1: "0 < len1" and len2: "0 < len2"
 begin
 
 lemma well_typed:
-  "seq_wt \<Gamma> (Bassign_trans C (Badd (Bsig A) (Bsig B)) 1)"
-  apply (rule seq_wt.intros(4))
-  apply (metis atype bexp_wt.intros(16) bexp_wt.intros(3) btype ctype len_def len1 len2)
-  done
+  "seq_wt \<Gamma> (Bassign_trans C (Bsub (Bsig A) (Bsig B)) 1)"
+  by (rule seq_wt.intros(4))
+     (metis atype bexp_wt.intros(20) bexp_wt.intros(3) btype ctype len_def len1 len2)
 
 abbreviation "lof_wline tw sig n \<equiv> lval_of (wline_of tw sig n)"
 
@@ -499,7 +492,7 @@ we are interested with for A should be the same as the index for B.\<close>
 definition property :: "nat \<Rightarrow> nat \<Rightarrow> sig assn2" where
   "property idxc idx =
       (\<lambda>tw. lof_wline tw C idxc =
-                  bin_to_bl len (sbl_to_bin (lof_wline tw A idx) + sbl_to_bin (lof_wline tw B idx)))"
+                  bin_to_bl len (sbl_to_bin (lof_wline tw A idx) - sbl_to_bin (lof_wline tw B idx)))"
 
 definition inv :: "sig assn2" where
   "inv tw \<equiv> (\<forall>i < fst tw. property (i + 1) i tw)"
@@ -511,7 +504,7 @@ abbreviation "next_world tw \<equiv> (next_time_world tw, snd tw)"
 
 lemma inv_next_time:
   assumes "inv tw"
-  assumes "beval_world_raw2 tw (Badd (Bsig A) (Bsig B)) v" and "type_of v = Lty Sig len"
+  assumes "beval_world_raw2 tw (Bsub (Bsig A) (Bsig B)) v" and "type_of v = Lty Sig len"
   defines "tw' \<equiv> tw[C, 1 :=\<^sub>2 v]"
   shows   "inv (next_time_world tw', snd tw')"
   unfolding inv_def
@@ -532,9 +525,9 @@ proof (rule, rule)
   { assume "i < fst tw"
     have "lof_wline tw' C (i + 1) = lof_wline tw C (i + 1)"
       by (metis \<open>i < get_time tw\<close> add_mono1 tw'_def worldline_upd2_before_dly)
-    also have "... = bin_to_bl len (sbl_to_bin (lof_wline tw A i) + sbl_to_bin (lof_wline tw B i))"
+    also have "... = bin_to_bl len (sbl_to_bin (lof_wline tw A i) - sbl_to_bin (lof_wline tw B i))"
       using assms(1) \<open>i < fst tw\<close> unfolding inv_def property_def by auto
-    also have "... = bin_to_bl len (sbl_to_bin (lof_wline tw' A i) + sbl_to_bin (lof_wline tw' B i))"
+    also have "... = bin_to_bl len (sbl_to_bin (lof_wline tw' A i) - sbl_to_bin (lof_wline tw' B i))"
       by (metis \<open>i < get_time tw\<close> add.commute trans_less_add2 tw'_def worldline_upd2_before_dly)
     finally have "property (i + 1) i (next_time_world tw', snd tw')"
       unfolding property_def by auto }
@@ -552,11 +545,11 @@ proof (rule, rule)
       less_add_one tw'_def worldline_upd2_before_dly)+
     moreover have "property (fst tw + 1) (fst tw) tw'"
     proof -
-      have assm2: "beval_world_raw (snd tw) (fst tw) (Badd (Bsig A) (Bsig B)) v"
+      have assm2: "beval_world_raw (snd tw) (fst tw) (Bsub (Bsig A) (Bsig B)) v"
         using assms(2) unfolding beval_world_raw2_def by auto
       have "wline_of tw' C (fst tw + 1) = v"
         unfolding tw'_def worldline_upd2_def worldline_upd_def by auto
-      also have "... =  Lv Sig (bin_to_bl_aux len (sbl_to_bin (lof_wline tw A (fst tw)) + sbl_to_bin (lof_wline tw B (fst tw))) [])"
+      also have "... =  Lv Sig (bin_to_bl_aux len (sbl_to_bin (lof_wline tw A (fst tw)) - sbl_to_bin (lof_wline tw B (fst tw))) [])"
         apply (rule beval_world_raw_cases[OF assm2])
         apply ( erule beval_cases)
         defer
@@ -564,7 +557,7 @@ proof (rule, rule)
         unfolding state_of_world_def using atype btype
         apply (metis assms(3) bin_to_bl_def comp_apply size_bin_to_bl ty.inject type_of.simps(2) val.sel(3))
         using assms(3) by auto
-      also have "... =  Lv Sig (bin_to_bl_aux len (sbl_to_bin (lof_wline tw' A (fst tw)) + sbl_to_bin (lof_wline tw' B (fst tw))) [])"
+      also have "... =  Lv Sig (bin_to_bl_aux len (sbl_to_bin (lof_wline tw' A (fst tw)) - sbl_to_bin (lof_wline tw' B (fst tw))) [])"
         by (metis Suc_eq_plus1 \<open>lval_of (wline_of tw' A i) = lval_of (wline_of tw' A (get_time tw))\<close>
         \<open>lval_of (wline_of tw' B i) = lval_of (wline_of tw' B (get_time tw))\<close> lessI tw'_def
         worldline_upd2_before_dly)
@@ -584,11 +577,11 @@ proof (rule, rule)
       by auto
     moreover have "property (fst tw + 1) (fst tw) tw'"
     proof -
-      have assm2: "beval_world_raw (snd tw) (fst tw) (Badd (Bsig A) (Bsig B)) v"
+      have assm2: "beval_world_raw (snd tw) (fst tw) (Bsub (Bsig A) (Bsig B)) v"
         using assms(2) unfolding beval_world_raw2_def by auto
       have "wline_of tw' C (fst tw + 1) = v"
         unfolding tw'_def worldline_upd2_def worldline_upd_def by auto
-      also have "... =  Lv Sig (bin_to_bl_aux len (sbl_to_bin (lof_wline tw A (fst tw)) + sbl_to_bin (lof_wline tw B (fst tw))) [])"
+      also have "... =  Lv Sig (bin_to_bl_aux len (sbl_to_bin (lof_wline tw A (fst tw)) - sbl_to_bin (lof_wline tw B (fst tw))) [])"
         apply (rule beval_world_raw_cases[OF assm2])
         apply ( erule beval_cases)
         defer
@@ -596,7 +589,7 @@ proof (rule, rule)
         unfolding state_of_world_def using atype btype
         apply (metis assms(3) bin_to_bl_def comp_def size_bin_to_bl ty.inject type_of.simps(2) val.sel(3))
         using assms(3) by auto
-      also have "... =  Lv Sig (bin_to_bl_aux len (sbl_to_bin (lof_wline tw' A (fst tw)) + sbl_to_bin (lof_wline tw' B (fst tw))) [])"
+      also have "... =  Lv Sig (bin_to_bl_aux len (sbl_to_bin (lof_wline tw' A (fst tw)) - sbl_to_bin (lof_wline tw' B (fst tw))) [])"
         by (metis less_add_one tw'_def worldline_upd2_before_dly)
       finally show ?thesis
         unfolding property_def bin_to_bl_def by auto
@@ -613,40 +606,40 @@ qed
 
 lemma type_correctness_length:
   assumes "wityping \<Gamma> (snd tw)"
-  assumes "beval_world_raw2 tw (Badd (Bsig A) (Bsig B)) v"
+  assumes "beval_world_raw2 tw (Bsub (Bsig A) (Bsig B)) v"
   shows   "type_of v = Lty Sig len"
 proof -
-  have "beval_world_raw (snd tw) (fst tw) (Badd (Bsig A) (Bsig B)) v"
+  have "beval_world_raw (snd tw) (fst tw) (Bsub (Bsig A) (Bsig B)) v"
     using assms(2) unfolding beval_world_raw2_def by auto
   have "type_of (state_of_world (snd tw) (fst tw) A) = Lty Sig len1" and
        "type_of (state_of_world (snd tw) (fst tw) B) = Lty Sig len2"
     using assms(1) unfolding wityping_def
     by (simp add: atype btype state_of_world_def wtyping_def)+
   show ?thesis
-    apply (rule beval_world_raw_cases[OF \<open>beval_world_raw (snd tw) (fst tw) (Badd (Bsig A) (Bsig B)) v\<close>])
+    apply (rule beval_world_raw_cases[OF \<open>beval_world_raw (snd tw) (fst tw) (Bsub (Bsig A) (Bsig B)) v\<close>])
     apply (erule beval_cases)
     apply (metis (no_types, hide_lams) \<open>type_of (state_of_world (snd tw) (get_time tw) A) = Lty Sig len1\<close> beval_cases(1) signedness.distinct(5) ty.inject type_of.simps(2))
     apply (metis \<open>type_of (state_of_world (snd tw) (get_time tw) A) = Lty Sig len1\<close> \<open>type_of (state_of_world (snd tw) (get_time tw) B) = Lty Sig len2\<close> beval_cases(1) bin_to_bl_def len_def size_bin_to_bl ty.inject type_of.simps(2) val.sel(3))
     done
 qed
 
-lemma add_seq_hoare_next_time:
+lemma seq_hoare_next_time:
   "\<turnstile> [\<lambda>tw. inv tw \<and> wityping \<Gamma> (snd tw)]
-        Bassign_trans C (Badd (Bsig A) (Bsig B)) 1
+        Bassign_trans C (Bsub (Bsig A) (Bsig B)) 1
      [\<lambda>tw. inv (next_world tw)]"
   apply (rule Conseq2[where Q="\<lambda>tw. inv (next_world tw) \<and> wityping \<Gamma> (snd tw)", rotated 1], rule Assign2, simp)
   using inv_next_time type_correctness_length
   by (metis ctype snd_conv worldline_upd2_def worldline_upd_preserve_wityping)
 
-lemma add_seq_hoare_next_time0:
+lemma seq_hoare_next_time0:
   "\<turnstile> [\<lambda>tw. fst tw = 0 \<and> wityping \<Gamma> (snd tw)]
-        Bassign_trans C (Badd (Bsig A) (Bsig B)) 1
+        Bassign_trans C (Bsub (Bsig A) (Bsig B)) 1
      [\<lambda>tw. inv (next_world tw)]"
   apply (rule Conseq2[where Q="\<lambda>tw. inv (next_world tw) \<and> wityping \<Gamma> (snd tw)", rotated 1], rule Assign2, simp)
   using inv_next_time type_correctness_length unfolding inv_def
   by (metis ctype gr_implies_not0 snd_conv worldline_upd2_def worldline_upd_preserve_wityping)
 
-lemma add_conc_hoare:
+lemma conc_hoare:
   "\<And>tw. inv tw \<and> inv2 tw \<and> disjnt {A, B} (event_of tw) \<Longrightarrow> inv (next_world tw)"
 proof -
   fix tw
@@ -683,7 +676,7 @@ proof -
     unfolding inv_def by auto
 qed
 
-lemma add_conc_hoare2:
+lemma conc_hoare2:
   "\<And>tw. inv tw \<and> inv2 tw \<and> disjnt {A, B} (event_of tw) \<Longrightarrow> inv2 (next_world tw)"
 proof -
   fix tw
@@ -715,7 +708,7 @@ qed
 
 lemma inv2_next_time:
   fixes tw
-  assumes "beval_world_raw2 tw (Badd (Bsig A) (Bsig B)) v" and "type_of v = Lty Sig len"
+  assumes "beval_world_raw2 tw (Bsub (Bsig A) (Bsig B)) v" and "type_of v = Lty Sig len"
   defines "tw' \<equiv> tw[C, 1 :=\<^sub>2 v]"
   shows   "inv2 (next_time_world tw', snd tw')"
   unfolding inv2_def
@@ -766,7 +759,7 @@ proof (rule, rule, rule)
     finally show "wline_of (next_world tw') B ?t' = wline_of tw B (fst tw)"
       by auto
   qed
-  have assm2: "beval_world_raw (snd tw) (fst tw) (Badd (Bsig A) (Bsig B)) v"
+  have assm2: "beval_world_raw (snd tw) (fst tw) (Bsub (Bsig A) (Bsig B)) v"
     using assms(1) unfolding beval_world_raw2_def by auto
   have "wline_of (next_world tw') C (i + 1) = v"
   proof -
@@ -776,7 +769,7 @@ proof (rule, rule, rule)
     thus ?thesis
       by auto
   qed
-  also have "lval_of ... = bin_to_bl len (sbl_to_bin (lof_wline tw A (fst tw)) + sbl_to_bin (lof_wline tw B (fst tw)))"
+  also have "lval_of ... = bin_to_bl len (sbl_to_bin (lof_wline tw A (fst tw)) - sbl_to_bin (lof_wline tw B (fst tw)))"
     apply (rule beval_world_raw_cases[OF assm2])
     apply (erule beval_cases)
     defer
@@ -788,146 +781,146 @@ proof (rule, rule, rule)
     by auto
 qed
 
-lemma add_seq_hoare_next_time1:
-  shows "\<turnstile> [\<lambda>tw. wityping \<Gamma> (snd tw)] Bassign_trans C (Badd (Bsig A) (Bsig B)) 1 [\<lambda>tw. inv2 (next_time_world tw, snd tw)]"
+lemma seq_hoare_next_time1:
+  shows "\<turnstile> [\<lambda>tw. wityping \<Gamma> (snd tw)] Bassign_trans C (Bsub (Bsig A) (Bsig B)) 1 [\<lambda>tw. inv2 (next_time_world tw, snd tw)]"
   apply (rule Assign2_altI)
   using inv2_next_time type_correctness_length by blast
 
-lemma add_conc_hoare3:
-  "\<turnstile> \<lbrace>\<lambda>tw. (inv tw \<and> wityping \<Gamma> (snd tw)) \<and> inv2 tw\<rbrace> add \<lbrace>\<lambda>tw. inv (next_time_world tw, snd tw) \<and> inv2 (next_time_world tw, snd tw)\<rbrace>"
-  unfolding add_def
+lemma conc_hoare3:
+  "\<turnstile> \<lbrace>\<lambda>tw. (inv tw \<and> wityping \<Gamma> (snd tw)) \<and> inv2 tw\<rbrace> sub \<lbrace>\<lambda>tw. inv (next_time_world tw, snd tw) \<and> inv2 (next_time_world tw, snd tw)\<rbrace>"
+  unfolding sub_def
   apply (rule Single)
    apply (rule Conj)
     apply (rule strengthen_precondition)
   apply (rule strengthen_precondition)
-    apply (rule add_seq_hoare_next_time)
+    apply (rule seq_hoare_next_time)
   apply (rule strengthen_precondition)
    apply (rule strengthen_precondition)
    apply (rule strengthen_precondition2)
-   apply (rule add_seq_hoare_next_time1)
-  using add_conc_hoare add_conc_hoare2 by blast
+   apply (rule seq_hoare_next_time1)
+  using conc_hoare conc_hoare2 by blast
 
 lemma seq_wt_add:
-  "seq_wt \<Gamma> (Bassign_trans C (Badd (Bsig A) (Bsig B)) 1)"
+  "seq_wt \<Gamma> (Bassign_trans C (Bsub (Bsig A) (Bsig B)) 1)"
   using well_typed by blast
 
-lemma add_conc_hoare4:
-  "\<turnstile> \<lbrace>\<lambda>tw. (inv tw \<and> wityping \<Gamma> (snd tw)) \<and> inv2 tw\<rbrace> add \<lbrace>\<lambda>tw. (inv (next_time_world tw, snd tw) \<and> wityping \<Gamma> (snd tw)) \<and> inv2 (next_time_world tw, snd tw)\<rbrace>"
+lemma conc_hoare4:
+  "\<turnstile> \<lbrace>\<lambda>tw. (inv tw \<and> wityping \<Gamma> (snd tw)) \<and> inv2 tw\<rbrace> sub \<lbrace>\<lambda>tw. (inv (next_time_world tw, snd tw) \<and> wityping \<Gamma> (snd tw)) \<and> inv2 (next_time_world tw, snd tw)\<rbrace>"
   apply (rule Conj2)
    apply (rule Conj2)
-    apply (rule weaken_post_conc_hoare[OF _ add_conc_hoare3], blast)
+    apply (rule weaken_post_conc_hoare[OF _ conc_hoare3], blast)
    apply (rule strengthen_pre_conc_hoare[rotated])
-    apply (unfold add_def, rule single_conc_stmt_preserve_wityping_hoare)
+    apply (unfold sub_def, rule single_conc_stmt_preserve_wityping_hoare)
     apply (rule seq_wt_add)
    apply blast
-  apply (fold add_def, rule weaken_post_conc_hoare[OF _ add_conc_hoare3], blast)
+  apply (fold sub_def, rule weaken_post_conc_hoare[OF _ conc_hoare3], blast)
   done
 
-lemma add_conc_sim':
-  "\<turnstile>\<^sub>s \<lbrace>\<lambda>tw. (inv tw \<and> wityping \<Gamma> (snd tw)) \<and> inv2 tw\<rbrace> add \<lbrace>\<lambda>tw. (inv tw \<and> wityping \<Gamma> (snd tw)) \<and> inv2 tw\<rbrace>"
+lemma conc_sim':
+  "\<turnstile>\<^sub>s \<lbrace>\<lambda>tw. (inv tw \<and> wityping \<Gamma> (snd tw)) \<and> inv2 tw\<rbrace> sub \<lbrace>\<lambda>tw. (inv tw \<and> wityping \<Gamma> (snd tw)) \<and> inv2 tw\<rbrace>"
   apply (rule While)
-  apply (unfold snd_conv, rule add_conc_hoare4)
+  apply (unfold snd_conv, rule conc_hoare4)
   done
 
-lemma add_conc_sim2:
-  "\<turnstile>\<^sub>s \<lbrace>\<lambda>tw. (inv tw \<and> wityping \<Gamma> (snd tw)) \<and> inv2 tw\<rbrace> add \<lbrace>inv\<rbrace>"
-  using add_conc_sim' Conseq_sim by blast
+lemma conc_sim2:
+  "\<turnstile>\<^sub>s \<lbrace>\<lambda>tw. (inv tw \<and> wityping \<Gamma> (snd tw)) \<and> inv2 tw\<rbrace> sub \<lbrace>inv\<rbrace>"
+  using conc_sim' Conseq_sim by blast
 
-lemma init_sat_add_inv:
-  "init_sim_hoare (\<lambda>tw. fst tw = 0 \<and> wityping \<Gamma> (snd tw)) add (\<lambda>tw. inv tw \<and> wityping \<Gamma> (snd tw))"
-  unfolding add_def
+lemma init_sat_inv:
+  "init_sim_hoare (\<lambda>tw. fst tw = 0 \<and> wityping \<Gamma> (snd tw)) sub (\<lambda>tw. inv tw \<and> wityping \<Gamma> (snd tw))"
+  unfolding sub_def
   apply (rule AssignI)
   apply (rule SingleI)
   apply (rule Conj)
-  unfolding snd_conv apply(rule add_seq_hoare_next_time0)
+  unfolding snd_conv apply(rule seq_hoare_next_time0)
   apply (rule strengthen_precondition2)
   by (metis seq_stmt_preserve_wityping_hoare well_typed)
 
-lemma init_sat_add_inv2:
-  "init_sim_hoare (\<lambda>tw. wityping \<Gamma> (snd tw)) add inv2"
-  unfolding add_def
+lemma init_sat_inv2:
+  "init_sim_hoare (\<lambda>tw. wityping \<Gamma> (snd tw)) sub inv2"
+  unfolding sub_def
   apply (rule AssignI)
   apply (rule SingleI)
-  unfolding snd_conv apply (rule add_seq_hoare_next_time1)
+  unfolding snd_conv apply (rule seq_hoare_next_time1)
   done
 
-lemma init_sat_add_inv_comb:
-  shows "init_sim_hoare (\<lambda>tw. fst tw = 0 \<and> wityping \<Gamma> (snd tw)) add  (\<lambda>tw. (inv tw \<and> wityping \<Gamma> (snd tw)) \<and> inv2 tw)"
+lemma init_sat_inv_comb:
+  shows "init_sim_hoare (\<lambda>tw. fst tw = 0 \<and> wityping \<Gamma> (snd tw)) sub  (\<lambda>tw. (inv tw \<and> wityping \<Gamma> (snd tw)) \<and> inv2 tw)"
   apply (rule ConjI_sim)
-  apply (rule init_sat_add_inv)
+  apply (rule init_sat_inv)
   apply (rule ConseqI_sim[rotated])
-  apply (rule init_sat_add_inv2)
+  apply (rule init_sat_inv2)
   by blast+
 
-lemma add_correctness:
-  assumes "sim_fin w (i + 1) add tw'" and "wityping \<Gamma> w"
+lemma correctness:
+  assumes "sim_fin w (i + 1) sub tw'" and "wityping \<Gamma> w"
   shows   "property (i + 1) i tw'"
 proof -
-  obtain tw where "init_sim (0, w) add tw" and  "tw, i + 1, add \<Rightarrow>\<^sub>S tw'"
+  obtain tw where "init_sim (0, w) sub tw" and  "tw, i + 1, sub \<Rightarrow>\<^sub>S tw'"
     using premises_sim_fin_obt[OF assms(1)] by auto
   hence "i + 1 < fst tw'"
     using world_maxtime_lt_fst_tres  by blast
-  have "conc_stmt_wf add"
-    unfolding conc_stmt_wf_def add_def by auto
-  moreover have "nonneg_delay_conc add"
-    unfolding add_def by auto
-  ultimately have "init_sim_valid (\<lambda>tw. fst tw = 0 \<and> wityping \<Gamma> (snd tw)) add (\<lambda>tw. (inv tw \<and> wityping \<Gamma> (snd tw)) \<and> inv2 tw)"
-    using init_sim_hoare_soundness[OF init_sat_add_inv_comb]
-    by (metis (no_types, lifting) conc_wt_cases(1) init_sat_add_inv_comb
-    init_sim_hoare_soundness add_def strengthen_precondition_init_sim_hoare)
+  have "conc_stmt_wf sub"
+    unfolding conc_stmt_wf_def sub_def by auto
+  moreover have "nonneg_delay_conc sub"
+    unfolding sub_def by auto
+  ultimately have "init_sim_valid (\<lambda>tw. fst tw = 0 \<and> wityping \<Gamma> (snd tw)) sub (\<lambda>tw. (inv tw \<and> wityping \<Gamma> (snd tw)) \<and> inv2 tw)"
+    using init_sim_hoare_soundness[OF init_sat_inv_comb]
+    by (metis (no_types, lifting) conc_wt_cases(1) init_sat_inv_comb
+    init_sim_hoare_soundness sub_def strengthen_precondition_init_sim_hoare)
   hence "inv tw \<and> wityping \<Gamma> (snd tw) \<and> inv2 tw"
-    using \<open>init_sim (0, w) add tw\<close> fst_conv assms(2) unfolding init_sim_valid_def
+    using \<open>init_sim (0, w) sub tw\<close> fst_conv assms(2) unfolding init_sim_valid_def
     by (metis snd_conv)
   hence "inv tw" and "inv2 tw" and "wityping \<Gamma> (snd tw)"
     by auto
-  moreover have "\<Turnstile>\<^sub>s \<lbrace>\<lambda>tw. (inv tw \<and> wityping \<Gamma> (snd tw)) \<and> inv2 tw\<rbrace> add \<lbrace>inv\<rbrace>"
-    using conc_sim_soundness[OF add_conc_sim2] \<open>conc_stmt_wf add\<close> \<open>nonneg_delay_conc add\<close>
+  moreover have "\<Turnstile>\<^sub>s \<lbrace>\<lambda>tw. (inv tw \<and> wityping \<Gamma> (snd tw)) \<and> inv2 tw\<rbrace> sub \<lbrace>inv\<rbrace>"
+    using conc_sim_soundness[OF conc_sim2] \<open>conc_stmt_wf sub\<close> \<open>nonneg_delay_conc sub\<close>
     by auto
   ultimately have "inv tw'"
-    using \<open>tw, i + 1, add \<Rightarrow>\<^sub>S tw'\<close> unfolding sim_hoare_valid_def by blast
+    using \<open>tw, i + 1, sub \<Rightarrow>\<^sub>S tw'\<close> unfolding sim_hoare_valid_def by blast
   with \<open>i + 1 < fst tw'\<close> show ?thesis
     unfolding inv_def by auto
 qed
 
-lemma add_correctness2:
-  assumes "sim_fin w (i + 1) add tw'" and "wityping \<Gamma> w"
+lemma correctness2:
+  assumes "sim_fin w (i + 1) sub tw'" and "wityping \<Gamma> w"
   shows   "wityping \<Gamma> (snd tw')"
 proof -
-  obtain tw where "init_sim (0, w) add tw" and  "tw, i + 1, add \<Rightarrow>\<^sub>S tw'"
+  obtain tw where "init_sim (0, w) sub tw" and  "tw, i + 1, sub \<Rightarrow>\<^sub>S tw'"
     using premises_sim_fin_obt[OF assms(1)] by auto
   hence "i + 1 < fst tw'"
     using world_maxtime_lt_fst_tres  by blast
-  have "conc_stmt_wf add"
-    unfolding conc_stmt_wf_def add_def by auto
-  moreover have "nonneg_delay_conc add"
-    unfolding add_def by auto
-  ultimately have "init_sim_valid (\<lambda>tw. fst tw = 0 \<and> wityping \<Gamma> (snd tw)) add (\<lambda>tw. (inv tw \<and> wityping \<Gamma> (snd tw)) \<and> inv2 tw)"
-    using init_sim_hoare_soundness[OF init_sat_add_inv_comb]
-    by (metis (no_types, lifting) conc_wt_cases(1) init_sat_add_inv_comb
-    init_sim_hoare_soundness add_def strengthen_precondition_init_sim_hoare)
+  have "conc_stmt_wf sub"
+    unfolding conc_stmt_wf_def sub_def by auto
+  moreover have "nonneg_delay_conc sub"
+    unfolding sub_def by auto
+  ultimately have "init_sim_valid (\<lambda>tw. fst tw = 0 \<and> wityping \<Gamma> (snd tw)) sub(\<lambda>tw. (inv tw \<and> wityping \<Gamma> (snd tw)) \<and> inv2 tw)"
+    using init_sim_hoare_soundness[OF init_sat_inv_comb]
+    by (metis (no_types, lifting) conc_wt_cases(1) init_sat_inv_comb
+    init_sim_hoare_soundness sub_def strengthen_precondition_init_sim_hoare)
   hence "inv tw \<and> wityping \<Gamma> (snd tw) \<and> inv2 tw"
-    using \<open>init_sim (0, w) add tw\<close> fst_conv assms(2) unfolding init_sim_valid_def
+    using \<open>init_sim (0, w) sub tw\<close> fst_conv assms(2) unfolding init_sim_valid_def
     by (metis snd_conv)
   hence "inv tw" and "inv2 tw" and "wityping \<Gamma> (snd tw)"
     by auto
-  moreover have "\<Turnstile>\<^sub>s \<lbrace>\<lambda>tw. (inv tw \<and> wityping \<Gamma> (snd tw)) \<and> inv2 tw\<rbrace> add \<lbrace>\<lambda>tw. wityping \<Gamma> (snd tw)\<rbrace>"
-    using conc_sim_soundness[OF add_conc_sim'] \<open>conc_stmt_wf add\<close> \<open>nonneg_delay_conc add\<close>
+  moreover have "\<Turnstile>\<^sub>s \<lbrace>\<lambda>tw. (inv tw \<and> wityping \<Gamma> (snd tw)) \<and> inv2 tw\<rbrace> sub \<lbrace>\<lambda>tw. wityping \<Gamma> (snd tw)\<rbrace>"
+    using conc_sim_soundness[OF conc_sim'] \<open>conc_stmt_wf sub\<close> \<open>nonneg_delay_conc sub\<close>
     by (metis (no_types, lifting) sim_hoare_valid_def)
   ultimately show "wityping \<Gamma> (snd tw')"
-    using \<open>tw, i + 1, add \<Rightarrow>\<^sub>S tw'\<close> unfolding sim_hoare_valid_def by blast
+    using \<open>tw, i + 1, sub \<Rightarrow>\<^sub>S tw'\<close> unfolding sim_hoare_valid_def by blast
 qed
 
-corollary add_correctness3:
-  assumes "sim_fin w (i + 1) add tw'" and "wityping \<Gamma> w"
+corollary correctness3:
+  assumes "sim_fin w (i + 1) sub tw'" and "wityping \<Gamma> w"
   defines "bsA \<equiv> lof_wline tw' A i"
   defines "bsB \<equiv> lof_wline tw' B i"
   defines "bsC \<equiv> lof_wline tw' C (i + 1)"
   assumes "0 < len1" and "0 < len2" \<comment> \<open>bit length of less than two is senseless for signed number\<close>
-  shows   "sbl_to_bin bsC mod 2 ^  len = (sbl_to_bin bsA + sbl_to_bin bsB) mod 2 ^ len" and
+  shows   "sbl_to_bin bsC mod 2 ^  len = (sbl_to_bin bsA - sbl_to_bin bsB) mod 2 ^ len" and
           "length bsC = len" and "0 < length bsB" and  "length bsA = len1"
 proof -
   have "property (i + 1) i tw'" and "wityping \<Gamma> (snd tw')"
-    using add_correctness[OF assms(1-2)] add_correctness2[OF assms(1-2)] by auto
+    using correctness[OF assms(1-2)] correctness2[OF assms(1-2)] by auto
   hence "length bsA = len1" and "length bsB = len2"
     by (smt assms(3-4) atype btype o_apply ty.distinct(1) ty.inject type_of.elims val.sel(3)
     wityping_def wtyping_def)+
@@ -936,25 +929,25 @@ proof -
   hence "0 < len"
     using assms unfolding len_def by auto
   have "lof_wline tw' C (i + 1) =
-                  bin_to_bl len (sbl_to_bin (lof_wline tw' A i) + sbl_to_bin (lof_wline tw' B i))"
+                  bin_to_bl len (sbl_to_bin (lof_wline tw' A i) - sbl_to_bin (lof_wline tw' B i))"
     using \<open>property (i + 1) i tw'\<close> unfolding property_def by auto
-  hence "bsC = bin_to_bl len (sbl_to_bin bsA + sbl_to_bin bsB)" (is "_ = ?rhs")
+  hence "bsC = bin_to_bl len (sbl_to_bin bsA - sbl_to_bin bsB)" (is "_ = ?rhs")
     unfolding bsA_def bsB_def bsC_def by auto
   hence "sbl_to_bin bsC = sbl_to_bin ?rhs"
     by auto
   hence "sbl_to_bin bsC mod 2 ^ len = sbl_to_bin ?rhs mod 2 ^ len"
     by auto
-  also have "... = (sbl_to_bin bsA + sbl_to_bin bsB) mod 2 ^ len"
+  also have "... = (sbl_to_bin bsA - sbl_to_bin bsB) mod 2 ^ len"
     using sbin_bl_bin' \<open>0 < len\<close> by auto
-  finally show "sbl_to_bin bsC mod 2 ^ len = (sbl_to_bin bsA + sbl_to_bin bsB) mod 2 ^ len"
+  finally show "sbl_to_bin bsC mod 2 ^ len = (sbl_to_bin bsA - sbl_to_bin bsB) mod 2 ^ len"
     by auto
   show "length bsC = len" and "0 < length bsB" and "length bsA = len1"
-    using \<open>bsC = bin_to_bl len (sbl_to_bin bsA + sbl_to_bin bsB)\<close> size_bin_to_bl \<open>0 < length bsB\<close>
+    using \<open>bsC = bin_to_bl len (sbl_to_bin bsA - sbl_to_bin bsB)\<close> size_bin_to_bl \<open>0 < length bsB\<close>
     \<open>length bsA = len1\<close> by blast+
 qed
 
-corollary add_correctness4:
-  assumes "sim_fin w (i + 1) add tw'" and "wityping \<Gamma> w"
+corollary correctness4:
+  assumes "sim_fin w (i + 1) sub tw'" and "wityping \<Gamma> w"
   defines "bsA \<equiv> lof_wline tw' A i"
   defines "bsB \<equiv> lof_wline tw' B i"
   defines "bsC \<equiv> lof_wline tw' C (i + 1)"
@@ -962,11 +955,11 @@ corollary add_correctness4:
   defines "repA \<equiv> - (int \<circ> of_bool) (hd bsA) * 2 ^ (length bsA - 1) + (\<Sum>i = 0..<length bsA - 1. (int \<circ> of_bool) (rev (tl bsA) ! i) * 2 ^ i)"
   defines "repB \<equiv> - (int \<circ> of_bool) (hd bsB) * 2 ^ (length bsB - 1) + (\<Sum>i = 0..<length bsB - 1. (int \<circ> of_bool) (rev (tl bsB) ! i) * 2 ^ i)"
   defines "repC \<equiv> - (int \<circ> of_bool) (hd bsC) * 2 ^ (length bsC - 1) + (\<Sum>i = 0..<length bsC - 1. (int \<circ> of_bool) (rev (tl bsC) ! i) * 2 ^ i)"
-  shows   "repC mod 2 ^ len = (repA + repB) mod 2 ^ len"
+  shows   "repC mod 2 ^ len = (repA - repB) mod 2 ^ len"
 proof -
   have "sbl_to_bin bsC mod 2 ^ len = 
-       (sbl_to_bin bsA + sbl_to_bin bsB) mod 2 ^ len" and  "length bsC = len" and "0 < length bsB" and "length bsA = len1"
-    using add_correctness3 assms by auto
+       (sbl_to_bin bsA - sbl_to_bin bsB) mod 2 ^ len" and  "length bsC = len" and "0 < length bsB" and "length bsA = len1"
+    using correctness3 assms by auto
   hence "0 < length bsC"
     unfolding len_def using \<open>0 < len1\<close> \<open>0 < len2\<close> by auto
   then obtain c bsC' where "bsC = c # bsC'" and "hd bsC = c" and "tl bsC = bsC'"
@@ -981,8 +974,6 @@ proof -
     using sbl_to_bin_correctness by simp+
   show ?thesis
     using \<open>sbl_to_bin bsC mod 2 ^ len = 
-       (sbl_to_bin bsA + sbl_to_bin bsB) mod 2 ^ len\<close> unfolding sA sB sC repA_def repB_def repC_def
+       (sbl_to_bin bsA - sbl_to_bin bsB) mod 2 ^ len\<close> unfolding sA sB sC repA_def repB_def repC_def
     by  metis 
 qed
-
-end
