Bits_Int_Aux.thy
@@ -10,7 +10,7 @@
 
 theory Bits_Int_Aux
   imports
-    Main "HOL-Word.Word"
+    Main "HOL-Word.Word" "HOL.Archimedean_Field"
 begin
 
 text \<open>The function @{term "bl_to_bin_aux"} is the auxiliary function for converting a bit vector
@@ -183,6 +183,212 @@ proof -
     finally show ?thesis
       by auto
   qed
+  finally show ?thesis
+    by auto
+qed
+
+lemma sbin_bl_bin':
+  assumes "0 < n"
+  shows   "sbl_to_bin (bin_to_bl n w) mod 2 ^ n = w mod 2 ^ n"
+proof -
+  obtain a bs where "bin_to_bl n w = (a # bs)"
+    using assms  size_bin_to_bl  by (metis list.size(3) not_less_zero sbl_to_bin.cases)
+  have "sbl_to_bin (bin_to_bl n w) = sbl_to_bin (a # bs)"
+    using \<open>bin_to_bl n w = (a # bs)\<close> by auto
+  also have "... = - (int o of_bool) a * 2 ^ (length bs)
+                 + (\<Sum>i = 0 ..< length bs. ((int o of_bool) (rev bs ! i)) * 2 ^ i)"
+    unfolding sbl_to_bin_correctness by auto
+  finally have "sbl_to_bin (bin_to_bl n w) = - (int o of_bool) a * 2 ^ (length bs)
+                                           + (\<Sum>i = 0 ..< length bs. ((int o of_bool) (rev bs ! i)) * 2 ^ i)"
+    by auto
+  have "sbl_to_bin (bin_to_bl n w) = sbl_to_bin (a # bs)"
+    using \<open>bin_to_bl n w = a # bs\<close> by auto
+  also have "... = bl_to_bin (a # bs) - (int o of_bool) a * 2 ^ (1 + length bs)"
+    by auto
+  also have "... = bl_to_bin (bin_to_bl n w) - (int o of_bool) a * 2 ^ (1 + length bs)"
+    using \<open>bin_to_bl n w = a # bs\<close> by auto
+  also have "... = bintrunc n w - (int o of_bool) a * 2 ^ (1 + length bs)"
+    unfolding bin_bl_bin by auto
+  also have "... = w mod (2 ^ n) - (int o of_bool) a * 2 ^ (1 + length bs)"
+    by (simp add: no_bintr_alt1)
+  also have "... = w mod (2 ^ n) - (int o of_bool) a * 2 ^ n"
+    by (metis \<open>bin_to_bl n w = a # bs\<close> length_Cons plus_1_eq_Suc size_bin_to_bl)
+  finally have "sbl_to_bin (bin_to_bl n w) = w mod (2 ^ n) - (int o of_bool) a * 2 ^ n"
+    by auto
+  hence "sbl_to_bin (bin_to_bl n w) mod 2 ^ n = (w mod 2 ^ n - (int o of_bool) a * 2 ^ n) mod 2 ^ n"
+    by auto
+  also have "... = (w - (int \<circ> of_bool) a * 2 ^ n) mod 2 ^ n"
+    using pull_mods(6)[where a="w" and c="2 ^ n" and b="(int o of_bool) a * 2 ^ n"] by auto
+  also have "... = w mod 2 ^ n"
+    by simp
+  finally show ?thesis
+    by auto
+qed
+
+lemma butlast_pow_rest_bl2bin:
+  "bl_to_bin ((butlast ^^ n) bl) = (bin_rest ^^ n) (bl_to_bin bl)"
+  by (simp add: bin_rest_bl_to_bin fn_comm_power')
+
+lemma take_rest_bl2bin:
+  "bl_to_bin (take (length bl - n) bl) = (bin_rest ^^ n) (bl_to_bin bl)"
+  by (metis butlast_pow_rest_bl2bin butlast_power)
+
+lemma bin_rest_compow:
+  "(bin_rest ^^ m) n = (n div 2 ^ m)"
+  using bin_rest_shiftr shiftr_int_def by (induct m) auto
+
+lemma bin_rest_sbl_to_bin:
+  assumes "1 < length bs"
+  shows "bin_rest (sbl_to_bin bs) = sbl_to_bin (butlast bs)"
+proof -
+  have "sbl_to_bin bs = bl_to_bin bs - (int o of_bool) (hd bs) * 2 ^ (length bs)"
+    using assms  by (metis (full_types) list.size(3) not_less_zero sbl_to_bin.elims)
+  hence "bin_rest (sbl_to_bin bs) = bin_rest (bl_to_bin bs + - (int o of_bool) (hd bs) * 2 ^ length bs)"
+    by auto
+  also have "... = bin_rest (bl_to_bin bs) - bin_rest ((int o of_bool) (hd bs) * 2 ^ length bs)"
+  proof -
+    have "2 dvd - (int \<circ> of_bool) (hd bs) * 2 ^ length bs"
+      using assms by auto
+    thus ?thesis
+      unfolding bin_rest_def  using div_plus_div_distrib_dvd_right  
+      by (smt dvd_neg_div mult_minus_left)
+  qed
+  also have "... = bl_to_bin (butlast bs) - (int o of_bool) (hd bs) * 2 ^ (length bs - 1)"
+    unfolding bin_rest_bl_to_bin bin_rest_def 
+    by (smt BIT_special_simps(3) assms bin_rest_BIT bin_rest_bl_to_bin bin_rest_def
+    mult_BIT_simps(1) mult_cancel_left2 mult_cancel_right2 not_less_zero o_apply of_bool_eq(1)
+    of_bool_eq(2) of_nat_1 power_eq_if semiring_1_class.of_nat_0)
+  also have "... = bl_to_bin (butlast bs) - (int o of_bool) (hd (butlast bs)) * 2 ^ (length (butlast bs))"
+    using assms hd_butlast by auto
+  also have "... = sbl_to_bin (butlast bs)"
+    by (metis assms length_butlast length_greater_0_conv sbl_to_bin.elims zero_less_diff)
+  finally show ?thesis
+    by auto
+qed
+
+lemma butlast_pow_rest_sbl2bin:
+  assumes "n < length bl" 
+  shows   "sbl_to_bin ((butlast ^^ n) bl) = (bin_rest ^^ n) (sbl_to_bin bl)"
+proof -
+  let ?bs = "(butlast ^^ n) bl"
+  have "(butlast ^^ n) bl \<noteq> []"
+    using assms unfolding butlast_power by auto
+  hence "sbl_to_bin ?bs = bl_to_bin ?bs - (int o of_bool) (hd ?bs) * 2 ^ (length ?bs)"
+    by (metis sbl_to_bin.elims)
+  moreover have "hd ?bs = hd bl"
+    unfolding butlast_power  by (simp add: assms)
+  moreover have "length ?bs = length bl - n"
+    unfolding butlast_power by simp
+  ultimately have "sbl_to_bin ?bs = bl_to_bin ?bs - (int o of_bool) (hd bl) * 2 ^ (length bl - n)"
+    by auto
+  also have "... = (bin_rest ^^ n) (bl_to_bin bl) - (int o of_bool) (hd bl) * 2 ^ (length bl - n)"
+    unfolding butlast_pow_rest_bl2bin by auto
+  also have "... = (bin_rest ^^ n) (bl_to_bin bl) + (- (int o of_bool) (hd bl) * 2 ^ length bl) div 2 ^ n"
+  proof -
+    have "(2::int) ^ (length bl - n) = 2 ^ length bl div 2 ^ n"
+      using power_diff[OF _ less_imp_le[OF assms], of "2::int"] by auto
+    hence "(int o of_bool) (hd bl) * 2 ^ (length bl - n) = (int o of_bool) (hd bl) * 2 ^ length bl div 2 ^ n"
+      by auto
+    thus ?thesis
+      by (smt add_diff_inverse_nat assms dvd_neg_div dvd_triv_left linorder_not_less
+      mult_cancel_right2 mult_minus_left o_apply of_bool_eq(1) of_bool_eq(2) of_nat_1
+      order_less_imp_le power_add semiring_1_class.of_nat_0)
+  qed
+  also have "... = (bin_rest ^^ n) (bl_to_bin bl) + (bin_rest ^^ n) (- (int o of_bool) (hd bl) * 2 ^ length bl)"
+    unfolding bin_rest_compow by auto
+  also have "... = (bin_rest ^^ n) (bl_to_bin bl - (int o of_bool) (hd bl) * 2 ^ length bl)"
+  proof -
+    have "2 ^ n dvd (- (int \<circ> of_bool) (hd bl) * 2 ^ length bl)"
+      using assms  dvd_triv_right order_less_imp_le power_le_dvd by blast
+    thus ?thesis
+      unfolding bin_rest_compow 
+      by (metis add.inverse_inverse diff_minus_eq_add div_plus_div_distrib_dvd_right
+          mult_minus_left)
+  qed
+  also have "... = (bin_rest ^^ n) (sbl_to_bin bl)"
+    by (metis (full_types) assms length_0_conv less_imp_diff_less less_not_refl2 sbl_to_bin.elims
+    zero_less_diff)
+  finally show ?thesis
+    by auto
+qed
+    
+lemma take_rest_sbl2bin:
+  assumes "n < length bl" 
+  shows   "sbl_to_bin (take (length bl - n) bl) = (bin_rest ^^ n) (sbl_to_bin bl)"
+  using butlast_pow_rest_sbl2bin[OF assms] by (simp add: butlast_power)
+
+lemma bl_to_bin_replicate_T:
+  "bl_to_bin (replicate n True) = 2 ^ n - 1"
+proof -
+  have "bl_to_bin (replicate n True) = (\<Sum>i = 0..<n. (int \<circ> of_bool) ((replicate n True) ! i) * 2 ^ i)"
+    unfolding bl_to_bin_correctness by auto
+  also have "... = 2 ^ n - 1"
+  proof (induction n)
+    case 0
+    then show ?case by auto
+  next
+    case (Suc n)
+    have " (\<Sum>i = 0..<Suc n. (int \<circ> of_bool) (replicate (Suc n) True ! i) * 2 ^ i) = 
+           (\<Sum>i = 0..<n. (int \<circ> of_bool) (replicate (Suc n) True ! i) * 2 ^ i) + 2 ^ n"
+      by (metis (no_types, lifting) One_nat_def add_Suc add_diff_cancel_left' lessI nth_replicate
+      o_apply of_bool_eq(2) of_nat_1 plus_1_eq_Suc power_0 power_add sum.atLeast0_lessThan_Suc)
+    also have "... = (\<Sum>i = 0..<n. (int \<circ> of_bool) (replicate n True ! i) * 2 ^ i) + 2 ^ n"
+      by (metis (no_types, lifting) Diff_cancel atLeastLessThan_iff empty_iff finite_atLeastLessThan
+      inf.idem less_Suc_eq nth_replicate sum.mono_neutral_cong)
+    also have "... = 2 ^ n - 1 + 2 ^ n"
+      using Suc by auto
+    also have "... = 2 ^ Suc n - 1"
+      by auto
+    finally show ?case by auto
+  qed
+  finally show ?thesis
+    by auto
+qed
+
+lemma sbl_to_bin_replicate_app:
+  assumes "0 < length bl"
+  shows "sbl_to_bin (replicate n (hd bl) @ bl) = sbl_to_bin bl"
+proof (cases "hd bl")
+  case False
+  hence "sbl_to_bin (replicate n (hd bl) @ bl) = sbl_to_bin (replicate n False @ bl)"
+    by auto
+  also have "... = bl_to_bin (replicate n False @ bl)"
+    using sbl_to_bin.simps assms 
+    by (smt False append_is_Nil_conv comp_apply hd_append hd_replicate length_greater_0_conv
+    mult_cancel_left of_bool_eq(1) power2_eq_square replicate_empty sbl_to_bin.elims
+    semiring_1_class.of_nat_0 zero_power2)
+  also have "... = bl_to_bin bl"
+    by (simp add: bl_to_bin_rep_F)
+  also have "... = sbl_to_bin bl"
+    using False sbl_to_bin.simps 
+    by (smt assms comp_apply length_greater_0_conv mult_cancel_left of_bool_eq(1) power2_eq_square
+        sbl_to_bin.elims semiring_1_class.of_nat_0 zero_power2)
+  finally show ?thesis 
+    by auto
+next
+  case True
+  hence "sbl_to_bin (replicate n (hd bl) @ bl) = sbl_to_bin (replicate n True @ bl)"
+    by auto
+  also have "... = bl_to_bin (replicate n True @ bl) - 2 ^ (length bl + n)"
+    by (smt True add.commute assms comp_apply hd_append hd_replicate length_append
+    length_greater_0_conv length_replicate mult_cancel_right2 of_bool_eq(2) of_nat_1 replicate_empty
+    sbl_to_bin.elims)
+  also have "... = bl_to_bin_aux bl (bl_to_bin (replicate n True)) - 2 ^ (length bl + n)"
+    unfolding bl_to_bin_append by auto
+  also have "... = bl_to_bin_aux bl (2 ^ n - 1) - 2 ^ (length bl + n)"
+    unfolding bl_to_bin_replicate_T by auto
+  also have "... = (2 ^ n - 1) * 2 ^ length bl + (\<Sum>i = 0..<length bl. (int \<circ> of_bool) (rev bl ! i) * 2 ^ i) - 2 ^ (length bl + n)"
+    unfolding bl_to_bin_aux_correctness by auto
+  also have "... = (2 ^ (length bl + n) - 2 ^ length bl) + (\<Sum>i = 0..<length bl. (int \<circ> of_bool) (rev bl ! i) * 2 ^ i) - 2 ^ (length bl + n)"
+    by (simp add: mult.commute power_add right_diff_distrib)
+  also have "... = (\<Sum>i = 0..<length bl. (int \<circ> of_bool) (rev bl ! i) * 2 ^ i) - 2 ^ length bl" 
+    by auto
+  also have "... = bl_to_bin bl - 2 ^ length bl"
+    unfolding bl_to_bin_correctness by auto
+  also have "... = bl_to_bin bl - (int o of_bool) (hd bl) * 2 ^ length bl"
+    using True by simp
+  also have "... = sbl_to_bin bl"
+    by (metis assms length_greater_0_conv sbl_to_bin.elims)
   finally show ?thesis
     by auto
 qed
