Shift_Right_Hoare.thy
@@ -1,0 +1,966 @@
+(*
+ * Copyright 2019, NTU
+ *
+ * This software may be distributed and modified according to the terms of
+ * the BSD 2-Clause license. Note that NO WARRANTY is provided.
+ * See "LICENSE_BSD2.txt" for details.
+ *
+ *  Author: Albert Rizaldi, NTU Singapore
+ *)
+
+theory Shift_Right_Hoare
+  imports VHDL_Hoare_Complete Bits_Int_Aux
+begin
+
+datatype sig = IN | OUT
+
+definition shiftr :: "nat \<Rightarrow> sig conc_stmt" where
+  "shiftr n \<equiv> process {IN} : Bassign_trans OUT (Bshiftr (Bsig IN) n) 1"
+
+lemma potential_tyenv:
+  assumes "seq_wt \<Gamma> (Bassign_trans OUT (Bshiftl (Bsig IN) n) 1)"
+  shows "\<exists>len>0. \<Gamma> IN = Lty Uns len \<and> \<Gamma> OUT = Lty Uns len \<or> \<Gamma> IN = Lty Sig len \<and> \<Gamma> OUT = Lty Sig len"
+  by (rule seq_wt_cases(4)[OF assms])
+     (metis bexp_wt_cases(14) bexp_wt_cases(9))
+ 
+locale unsigned_shift_right =
+  fixes \<Gamma> :: "sig tyenv"
+  fixes len :: nat
+  fixes amount :: nat
+  assumes "0 < len"
+  assumes "\<Gamma> IN = Lty Uns len \<and> \<Gamma> OUT = Lty Uns len"
+begin
+
+lemma well_typed:
+  "seq_wt \<Gamma> (Bassign_trans OUT (Bshiftr (Bsig IN) n) 1)"
+  by (rule seq_wt.intros(4))
+     (smt bexp_wt.intros(23) bexp_wt.intros(24) bexp_wt.intros(3) unsigned_shift_right_axioms
+     unsigned_shift_right_def)
+
+abbreviation "lof_wline tw sig n \<equiv> lval_of (wline_of tw sig n)"
+
+text \<open>Here we factor out common expression in both inv1 and inv2. It is parametrised by the index
+we are interested with for C (first argument) and A (the second argument). Note that the index
+we are interested with for A should be the same as the index for B.\<close>
+
+definition property :: "nat \<Rightarrow> nat \<Rightarrow> sig assn2" where
+  "property idxc idx =
+      (\<lambda>tw. lof_wline tw OUT idxc = take len (replicate amount False @ lof_wline tw IN idx))"
+
+definition inv :: "sig assn2" where
+  "inv tw \<equiv> (\<forall>i < fst tw. property (i + 1) i tw)"
+
+definition inv2 :: "sig assn2" where
+  "inv2 tw \<equiv> (disjnt {IN} (event_of tw) \<longrightarrow> (\<forall>i \<ge> fst tw. property (i + 1) (fst tw) tw))"
+
+abbreviation "next_world tw \<equiv> (next_time_world tw, snd tw)"
+
+lemma inv_next_time:
+  assumes "inv tw"
+  assumes "beval_world_raw2 tw (Bshiftr (Bsig IN) amount) v" and "type_of v = Lty Uns len"
+  defines "tw' \<equiv> tw[OUT, 1 :=\<^sub>2 v]"
+  shows   "inv (next_time_world tw', snd tw')"
+  unfolding inv_def
+proof (rule, rule)
+  fix i
+  assume "i < fst (next_world tw')"
+  hence "i < next_time_world tw'"
+    by auto
+  have "fst tw' < next_time_world tw'"
+    using next_time_world_at_least  using nat_less_le by blast
+  moreover have "fst tw = fst tw'"
+    unfolding tw'_def worldline_upd2_def worldline_upd_def by auto
+  ultimately have "fst tw < next_time_world tw'"
+    by auto
+  hence "i < fst tw \<or> fst tw \<le> i \<and> i < next_time_world tw' - 1 \<or> i = next_time_world tw' - 1"
+    using \<open>i < next_time_world tw'\<close> by linarith
+  moreover
+  { assume "i < fst tw"
+    have "lof_wline tw' OUT (i + 1) = lof_wline tw OUT (i + 1)"
+      by (metis \<open>i < get_time tw\<close> add_mono1 tw'_def worldline_upd2_before_dly)
+    also have "... = take len (replicate amount False @ lof_wline tw IN i)"
+      using assms(1) \<open>i < fst tw\<close> unfolding inv_def property_def by auto
+    also have "... = take len (replicate amount False @ lof_wline tw' IN i)"
+      by (metis \<open>i < get_time tw\<close> add.commute trans_less_add2 tw'_def worldline_upd2_before_dly)
+    finally have "property (i + 1) i (next_time_world tw', snd tw')"
+      unfolding property_def by auto }
+  moreover
+  { assume "fst tw \<le> i \<and> i < next_time_world tw' - 1"
+    hence "fst tw \<le> i" and "i < next_time_world tw' - 1"
+      by auto
+    hence "lof_wline tw' OUT (i + 1) = lof_wline tw' OUT (fst tw + 1)"
+      using unchanged_until_next_time_world
+      by (metis (mono_tags, lifting) Suc_eq_plus1 \<open>get_time tw = get_time tw'\<close> le_Suc_eq le_add1
+          le_less_trans less_diff_conv)
+    moreover have "lof_wline tw' IN i = lof_wline tw' IN (fst tw)" 
+      using unchanged_until_next_time_world
+      by (metis \<open>get_time tw = get_time tw'\<close> \<open>get_time tw \<le> i\<close> \<open>i < next_time_world tw'\<close>)
+    moreover have "property (fst tw + 1) (fst tw) tw'"
+    proof -
+      have assm2: "beval_world_raw (snd tw) (fst tw) (Bshiftr (Bsig IN) amount) v"
+        using assms(2) unfolding beval_world_raw2_def by auto
+      have "wline_of tw' OUT (fst tw + 1) = v"
+        unfolding tw'_def worldline_upd2_def worldline_upd_def by auto
+      also have "... =  Lv Uns (take len (replicate amount False @ lof_wline tw IN (fst tw)))"
+        apply (rule beval_world_raw_cases[OF assm2])
+        apply ( erule_tac[!] beval_cases)+
+        unfolding state_of_world_def 
+        apply (metis assms(3) comp_eq_dest_lhs length_append length_replicate length_take min_minus
+               min_pm take_append take_replicate ty.inject type_of.simps(2) val.sel(3))
+        using assms(3) by auto
+      also have "... =  Lv Uns (take len (replicate amount False @ lof_wline tw' IN (fst tw)))"
+        by (metis less_add_one tw'_def worldline_upd2_before_dly)
+      finally show ?thesis
+        unfolding property_def bin_to_bl_def by auto
+    qed
+    ultimately have "property (i + 1) i (next_world tw')"
+      unfolding property_def by auto }
+  moreover
+  { assume "i = next_time_world tw' - 1"
+    hence "lof_wline tw' OUT (i + 1) = lof_wline tw' OUT (next_time_world tw')"
+      using \<open>i < next_time_world tw'\<close> by force
+    also have "... = lof_wline tw' OUT (fst tw + 1)"
+      using \<open>fst tw < next_time_world tw'\<close> unfolding tw'_def worldline_upd2_def
+      worldline_upd_def by auto
+    finally have "lof_wline tw' OUT (i + 1) = lof_wline tw' OUT (fst tw + 1)"
+      by auto
+    moreover have "property (fst tw + 1) (fst tw) tw'"
+    proof -
+      have assm2: "beval_world_raw (snd tw) (fst tw) (Bshiftr (Bsig IN) amount) v"
+        using assms(2) unfolding beval_world_raw2_def by auto
+      have "wline_of tw' OUT (fst tw + 1) = v"
+        unfolding tw'_def worldline_upd2_def worldline_upd_def by auto
+      also have "... =  Lv Uns (take len (replicate amount False @ lof_wline tw IN (fst tw)))"
+        apply (rule beval_world_raw_cases[OF assm2])
+        apply ( erule_tac[!] beval_cases)+
+        unfolding state_of_world_def 
+        apply (metis assms(3) comp_eq_dest_lhs length_append length_replicate length_take min_minus
+               min_pm take_append take_replicate ty.inject type_of.simps(2) val.sel(3))
+        using assms(3) by auto
+      also have "... =  Lv Uns (take len (replicate amount False @ lof_wline tw' IN (fst tw)))"
+        by (metis less_add_one tw'_def worldline_upd2_before_dly)
+      finally show ?thesis
+        unfolding property_def bin_to_bl_def by auto
+    qed
+    moreover have "lof_wline tw' IN i = lof_wline tw' IN (fst tw)"
+      using unchanged_until_next_time_world
+      by (metis \<open>get_time tw < next_time_world tw'\<close> \<open>get_time tw = get_time tw'\<close> \<open>i <
+      next_time_world tw'\<close> \<open>i = next_time_world tw' - 1\<close> add_le_imp_le_diff discrete)+
+    ultimately have "property (i + 1) i (next_world tw')"
+      unfolding property_def by auto }
+  ultimately show "property (i + 1) i (next_world tw')"
+    by auto
+qed
+
+lemma type_correctness_length:
+  assumes "wityping \<Gamma> (snd tw)"
+  assumes "beval_world_raw2 tw (Bshiftr (Bsig IN) amount) v"
+  shows   "type_of v = Lty Uns len"
+proof -
+  have "beval_world_raw (snd tw) (fst tw) (Bshiftr (Bsig IN) amount) v"
+    using assms(2) unfolding beval_world_raw2_def by auto
+  have *: "type_of (state_of_world (snd tw) (fst tw) IN) = Lty Uns len"    
+    using assms(1) unfolding wityping_def
+    by (metis state_of_world_def unsigned_shift_right_axioms unsigned_shift_right_def wtyping_def)
+  show ?thesis
+    apply (rule beval_world_raw_cases[OF \<open>beval_world_raw (snd tw) (fst tw) (Bshiftr (Bsig IN) amount) v\<close>])
+    apply (erule beval_cases)+
+    unfolding state_of_world_def 
+    apply (metis "*" length_append length_replicate length_take min_minus min_pm state_of_world_def type_of.simps(2))
+    apply (erule beval_cases)+
+    apply (metis "*" signedness.distinct(5) state_of_world_def ty.inject type_of.simps(2))
+    done
+qed
+
+lemma seq_hoare_next_time:
+  "\<turnstile> [\<lambda>tw. inv tw \<and> wityping \<Gamma> (snd tw)]
+        Bassign_trans OUT (Bshiftr (Bsig IN) amount) 1
+     [\<lambda>tw. inv (next_world tw)]"
+  apply (rule Conseq2[where Q="\<lambda>tw. inv (next_world tw) \<and> wityping \<Gamma> (snd tw)", rotated 1], rule Assign2, simp)
+  using inv_next_time type_correctness_length
+  by (metis BassignE_hoare2 seq_stmt_preserve_wityping_hoare well_typed)
+
+lemma seq_hoare_next_time0:
+  "\<turnstile> [\<lambda>tw. fst tw = 0 \<and> wityping \<Gamma> (snd tw)]
+        Bassign_trans OUT (Bshiftr (Bsig IN) amount) 1
+     [\<lambda>tw. inv (next_world tw)]"
+  apply (rule Conseq2[where Q="\<lambda>tw. inv (next_world tw) \<and> wityping \<Gamma> (snd tw)", rotated 1], rule Assign2, simp)
+  using inv_next_time type_correctness_length unfolding inv_def
+  by (metis BassignE_hoare2 gr_implies_not_zero seq_stmt_preserve_wityping_hoare well_typed)
+
+lemma conc_hoare:
+  "\<And>tw. inv tw \<and> inv2 tw \<and> disjnt {IN} (event_of tw) \<Longrightarrow> inv (next_world tw)"
+proof -
+  fix tw
+  assume "inv tw \<and> inv2 tw \<and> disjnt {IN} (event_of tw)"
+  hence "inv tw" and "inv2 tw" and "disjnt {IN} (event_of tw)"
+    by auto
+  { fix i
+    assume "i < next_time_world tw"
+    have "fst tw < next_time_world tw"
+      by (simp add: next_time_world_at_least)
+    have "i < fst tw \<or> fst tw \<le> i"
+      by auto
+    moreover
+    { assume "i < fst tw"
+      hence "property (i + 1) i tw"
+        using \<open>inv tw\<close> unfolding inv_def by auto
+      hence "property (i + 1) i (next_world tw)"
+        unfolding property_def by simp }
+    moreover
+    { assume "fst tw \<le> i"
+      moreover have "\<forall>i \<ge> fst tw. property (i + 1) (fst tw) tw"
+        using \<open>inv2 tw\<close> \<open>disjnt {IN} (event_of tw)\<close> unfolding inv2_def
+        by auto
+      ultimately have "property (i + 1) (fst tw) tw"
+        by auto
+      hence "property (i + 1) i tw"
+        unfolding property_def
+        by (metis \<open>get_time tw \<le> i\<close> \<open>i < next_time_world tw\<close> unchanged_until_next_time_world)
+      hence "property (i + 1) i (next_world tw)"
+        unfolding property_def by auto }
+    ultimately have "property (i + 1) i (next_world tw)"
+      by auto }
+  thus "inv (next_world tw)"
+    unfolding inv_def by auto
+qed
+
+lemma conc_hoare2:
+  "\<And>tw. inv tw \<and> inv2 tw \<and> disjnt {IN} (event_of tw) \<Longrightarrow> inv2 (next_world tw)"
+proof -
+  fix tw
+  assume "inv tw \<and> inv2 tw \<and> disjnt {IN} (event_of tw)"
+  hence "inv tw" and "inv2 tw" and "disjnt {IN} (event_of tw)"
+    by auto
+  let ?t' = "next_time_world tw"
+  { assume "disjnt {IN} (event_of (next_world tw))"
+    hence *: "lof_wline tw IN ?t' = lof_wline tw IN (?t' - 1)"
+      unfolding event_of_alt_def
+      by (smt comp_apply diff_0_eq_0 disjnt_insert1 fst_conv mem_Collect_eq snd_conv)
+    have "fst tw < ?t'"
+      by (simp add: next_time_world_at_least)
+    { fix i
+      assume "?t' \<le> i"
+      have "property (i + 1) (fst tw) tw"
+        using \<open>inv2 tw\<close> \<open>disjnt {IN} (event_of tw)\<close> unfolding inv2_def
+        using \<open>get_time tw < next_time_world tw\<close> \<open>next_time_world tw \<le> i\<close> by auto
+      moreover have "lof_wline tw IN (fst tw) = lof_wline tw IN (?t' - 1)"
+        by (metis \<open>get_time tw < next_time_world tw\<close> add_le_imp_le_diff diff_less discrete
+        gr_implies_not0 not_less_iff_gr_or_eq unchanged_until_next_time_world zero_less_one)
+      ultimately have "property (i + 1) ?t' (next_world tw)"
+        unfolding property_def using *  by auto }
+    hence "\<forall>i\<ge>?t'. property (i + 1) ?t' (next_world tw)"
+      by auto }
+  thus "inv2 (next_world tw)"
+    unfolding inv2_def by auto
+qed
+
+lemma inv2_next_time:
+  fixes tw
+  assumes "beval_world_raw2 tw (Bshiftr (Bsig IN) amount) v" and "type_of v = Lty Uns len"
+  defines "tw' \<equiv> tw[OUT, 1 :=\<^sub>2 v]"
+  shows   "inv2 (next_time_world tw', snd tw')"
+  unfolding inv2_def
+proof (rule, rule, rule)
+  fix i
+  assume "disjnt {IN} (event_of (next_world tw'))"
+  hence "IN \<notin> event_of (next_world tw')"
+    by auto
+  assume "fst (next_world tw') \<le> i"
+  hence "next_time_world tw' \<le> i"
+    by auto
+  let ?t' = "next_time_world tw'"
+  have "fst tw' < ?t'"
+    using next_time_world_at_least by blast
+  moreover have "fst tw = fst tw'"
+    unfolding tw'_def unfolding worldline_upd2_def by auto
+  ultimately have "fst tw < ?t'"
+    by auto
+  have 0: "wline_of (next_world tw') IN ?t' = wline_of tw IN (fst tw)"
+  proof -
+    have "wline_of tw' IN ?t' = wline_of tw' IN (?t' - 1)"
+      using \<open>IN \<notin> event_of (next_world tw')\<close> unfolding event_of_alt_def
+      using \<open>get_time tw' < next_time_world tw'\<close> by auto
+    also have " ... = wline_of tw' IN (fst tw')"
+      using unchanged_until_next_time_world
+      by (metis (no_types, lifting) Suc_diff_1 \<open>get_time tw' < next_time_world tw'\<close> diff_less
+      gr_implies_not_zero le_0_eq less_Suc_eq_le not_less zero_less_one)
+    also have "... = wline_of tw' IN (fst tw)"
+      by (simp add: \<open>get_time tw = get_time tw'\<close>)
+    also have "... = wline_of tw IN (fst tw)"
+      unfolding tw'_def worldline_upd2_def worldline_upd_def by auto
+    finally show "wline_of (next_world tw') IN ?t' = wline_of tw IN (fst tw)"
+      by auto
+  qed
+  have assm2: "beval_world_raw (snd tw) (fst tw) (Bshiftr (Bsig IN) amount) v"
+    using assms(1) unfolding beval_world_raw2_def by auto
+  have "wline_of (next_world tw') OUT (i + 1) = v"
+  proof -
+    have "wline_of tw' OUT (i + 1) = v"
+      using `fst tw < ?t'` \<open>?t' \<le> i\<close>
+      unfolding tw'_def worldline_upd2_def worldline_upd_def by auto
+    thus ?thesis
+      by auto
+  qed
+  also have "lval_of ... = take len (replicate amount False @ lof_wline tw IN (fst tw))"
+    apply (rule beval_world_raw_cases[OF assm2])
+    apply (erule_tac[!] beval_cases)+
+    apply (metis assms(2) comp_def length_append length_replicate length_take min_minus min_pm
+           state_of_world_def take_append take_replicate ty.inject type_of.simps(2) val.sel(3))
+    using assms(2) by auto
+  finally have "property (i + 1) ?t' (next_world tw')"
+    unfolding property_def using 0  by auto
+  thus "property (i + 1) (get_time (next_time_world tw', snd tw')) (next_time_world tw', snd tw')"
+    by auto
+qed
+
+lemma seq_hoare_next_time1:
+  shows "\<turnstile> [\<lambda>tw. wityping \<Gamma> (snd tw)] Bassign_trans OUT (Bshiftr (Bsig IN) amount) 1 [\<lambda>tw. inv2 (next_time_world tw, snd tw)]"
+  apply (rule Assign2_altI)
+  using inv2_next_time  type_correctness_length by blast
+
+lemma conc_hoare3:
+  "\<turnstile> \<lbrace>\<lambda>tw. (inv tw \<and> wityping \<Gamma> (snd tw)) \<and> inv2 tw\<rbrace> shiftr amount \<lbrace>\<lambda>tw. inv (next_time_world tw, snd tw) \<and> inv2 (next_time_world tw, snd tw)\<rbrace>"
+  unfolding shiftr_def
+  apply (rule Single)
+   apply (rule Conj)
+    apply (rule strengthen_precondition)
+  apply (rule strengthen_precondition)
+    apply (rule seq_hoare_next_time)
+  apply (rule strengthen_precondition)
+   apply (rule strengthen_precondition)
+   apply (rule strengthen_precondition2)
+   apply (rule seq_hoare_next_time1)
+  using conc_hoare conc_hoare2 by blast
+
+lemma seq_wt_sub:
+  "seq_wt \<Gamma> (Bassign_trans OUT (Bshiftr (Bsig IN) amount) 1)"
+  using well_typed by blast
+
+lemma conc_hoare4:
+  "\<turnstile> \<lbrace>\<lambda>tw. (inv tw \<and> wityping \<Gamma> (snd tw)) \<and> inv2 tw\<rbrace> shiftr amount \<lbrace>\<lambda>tw. (inv (next_time_world tw, snd tw) \<and> wityping \<Gamma> (snd tw)) \<and> inv2 (next_time_world tw, snd tw)\<rbrace>"
+  apply (rule Conj2)
+   apply (rule Conj2)
+    apply (rule weaken_post_conc_hoare[OF _ conc_hoare3], blast)
+   apply (rule strengthen_pre_conc_hoare[rotated])
+    apply (unfold shiftr_def, rule single_conc_stmt_preserve_wityping_hoare)
+    apply (rule seq_wt_sub)
+   apply blast
+  apply (fold shiftr_def, rule weaken_post_conc_hoare[OF _ conc_hoare3], blast)
+  done
+
+lemma conc_sim':
+  "\<turnstile>\<^sub>s \<lbrace>\<lambda>tw. (inv tw \<and> wityping \<Gamma> (snd tw)) \<and> inv2 tw\<rbrace> shiftr amount \<lbrace>\<lambda>tw. (inv tw \<and> wityping \<Gamma> (snd tw)) \<and> inv2 tw\<rbrace>"
+  apply (rule While)
+  apply (unfold snd_conv, rule conc_hoare4)
+  done
+
+lemma conc_sim2:
+  "\<turnstile>\<^sub>s \<lbrace>\<lambda>tw. (inv tw \<and> wityping \<Gamma> (snd tw)) \<and> inv2 tw\<rbrace> shiftr amount \<lbrace>inv\<rbrace>"
+  using conc_sim' Conseq_sim by blast
+
+lemma init_sat_inv:
+  "init_sim_hoare (\<lambda>tw. fst tw = 0 \<and> wityping \<Gamma> (snd tw)) (shiftr amount) (\<lambda>tw. inv tw \<and> wityping \<Gamma> (snd tw))"
+  unfolding shiftr_def
+  apply (rule AssignI)
+  apply (rule SingleI)
+  apply (rule Conj)
+  unfolding snd_conv apply(rule seq_hoare_next_time0)
+  apply (rule strengthen_precondition2)
+  by (metis seq_stmt_preserve_wityping_hoare well_typed)
+
+lemma init_sat_inv2:
+  "init_sim_hoare (\<lambda>tw. wityping \<Gamma> (snd tw)) (shiftr amount) inv2"
+  unfolding shiftr_def
+  apply (rule AssignI)
+  apply (rule SingleI)
+  unfolding snd_conv apply (rule seq_hoare_next_time1)
+  done
+
+lemma init_sat_inv_comb:
+  shows "init_sim_hoare (\<lambda>tw. fst tw = 0 \<and> wityping \<Gamma> (snd tw)) (shiftr amount)  (\<lambda>tw. (inv tw \<and> wityping \<Gamma> (snd tw)) \<and> inv2 tw)"
+  apply (rule ConjI_sim)
+  apply (rule init_sat_inv)
+  apply (rule ConseqI_sim[rotated])
+  apply (rule init_sat_inv2)
+  by blast+
+
+lemma correctness:
+  assumes "sim_fin w (i + 1) (shiftr amount) tw'" and "wityping \<Gamma> w"
+  shows   "property (i + 1) i tw'"
+proof -
+  obtain tw where "init_sim (0, w) (shiftr amount) tw" and  "tw, i + 1, shiftr amount \<Rightarrow>\<^sub>S tw'"
+    using premises_sim_fin_obt[OF assms(1)] by auto
+  hence "i + 1 < fst tw'"
+    using world_maxtime_lt_fst_tres  by blast
+  have "conc_stmt_wf (shiftr amount)"
+    unfolding conc_stmt_wf_def shiftr_def by auto
+  moreover have "nonneg_delay_conc (shiftr amount)"
+    unfolding shiftr_def by auto
+  ultimately have "init_sim_valid (\<lambda>tw. fst tw = 0 \<and> wityping \<Gamma> (snd tw)) (shiftr amount) (\<lambda>tw. (inv tw \<and> wityping \<Gamma> (snd tw)) \<and> inv2 tw)"
+    using init_sim_hoare_soundness[OF init_sat_inv_comb]
+    by (metis (no_types, lifting) conc_wt_cases(1) init_sat_inv_comb
+    init_sim_hoare_soundness sub_def strengthen_precondition_init_sim_hoare)
+  hence "inv tw \<and> wityping \<Gamma> (snd tw) \<and> inv2 tw"
+    using \<open>init_sim (0, w) (shiftr amount) tw\<close> fst_conv assms(2) unfolding init_sim_valid_def
+    by (metis snd_conv)
+  hence "inv tw" and "inv2 tw" and "wityping \<Gamma> (snd tw)"
+    by auto
+  moreover have "\<Turnstile>\<^sub>s \<lbrace>\<lambda>tw. (inv tw \<and> wityping \<Gamma> (snd tw)) \<and> inv2 tw\<rbrace> shiftr amount \<lbrace>inv\<rbrace>"
+    using conc_sim_soundness[OF conc_sim2] \<open>conc_stmt_wf (shiftr amount)\<close> \<open>nonneg_delay_conc (shiftr amount)\<close>
+    by auto
+  ultimately have "inv tw'"
+    using \<open>tw, i + 1, shiftr amount \<Rightarrow>\<^sub>S tw'\<close> unfolding sim_hoare_valid_def by blast
+  with \<open>i + 1 < fst tw'\<close> show ?thesis
+    unfolding inv_def by auto
+qed
+
+lemma correctness_wityping:
+  assumes "sim_fin w (i + 1) (shiftr amount) tw'" and "wityping \<Gamma> w"
+  shows   "wityping \<Gamma> (snd tw')"
+proof -
+  obtain tw where "init_sim (0, w) (shiftr amount) tw" and  "tw, i + 1, (shiftr amount) \<Rightarrow>\<^sub>S tw'"
+    using premises_sim_fin_obt[OF assms(1)] by auto
+  hence "i + 1 < fst tw'"
+    using world_maxtime_lt_fst_tres  by blast
+  have "conc_stmt_wf (shiftr amount)"
+    unfolding conc_stmt_wf_def shiftr_def by auto
+  moreover have "nonneg_delay_conc (shiftr amount)"
+    unfolding shiftr_def by auto
+  ultimately have "init_sim_valid (\<lambda>tw. fst tw = 0 \<and> wityping \<Gamma> (snd tw)) (shiftr amount) (\<lambda>tw. (inv tw \<and> wityping \<Gamma> (snd tw)) \<and> inv2 tw)"
+    using init_sim_hoare_soundness[OF init_sat_inv_comb]
+    by (metis (no_types, lifting) conc_wt_cases(1) init_sat_inv_comb
+    init_sim_hoare_soundness sub_def strengthen_precondition_init_sim_hoare)
+  hence "inv tw \<and> wityping \<Gamma> (snd tw) \<and> inv2 tw"
+    using \<open>init_sim (0, w) (shiftr amount) tw\<close> fst_conv assms(2) unfolding init_sim_valid_def
+    by (metis snd_conv)
+  hence "inv tw" and "inv2 tw" and "wityping \<Gamma> (snd tw)"
+    by auto
+  moreover have "\<Turnstile>\<^sub>s \<lbrace>\<lambda>tw. (inv tw \<and> wityping \<Gamma> (snd tw)) \<and> inv2 tw\<rbrace> (shiftr amount) \<lbrace>\<lambda>tw. wityping \<Gamma> (snd tw)\<rbrace>"
+    using conc_sim_soundness[OF conc_sim'] \<open>conc_stmt_wf (shiftr amount)\<close> \<open>nonneg_delay_conc (shiftr amount)\<close>
+    by (smt sim_hoare_valid_def)  
+  ultimately show "wityping \<Gamma> (snd tw')"
+    using \<open>tw, i + 1, (shiftr amount) \<Rightarrow>\<^sub>S tw'\<close> unfolding sim_hoare_valid_def by blast
+qed
+
+corollary correctness2:
+  assumes "sim_fin w (i + 1) (shiftr amount) tw'" and "wityping \<Gamma> w"
+  defines "bsIN  \<equiv> lof_wline tw' IN i"
+  defines "bsOUT \<equiv> lof_wline tw' OUT (i + 1)"
+  shows   "(\<Sum>i = 0..<length bsOUT. (int \<circ> of_bool) (rev bsOUT ! i) * 2 ^ i) =
+          ((\<Sum>i = 0..<length bsIN. (int \<circ> of_bool) (rev bsIN  ! i) * 2 ^ i) div (2 ^ amount)) "
+proof -
+  have "wityping \<Gamma> (snd tw')"
+    using correctness_wityping[OF assms(1-2)] by auto
+  hence "length bsIN = len"
+    by (smt assms(3) o_apply ty.distinct(1) ty.inject type_of.elims unsigned_shift_right_axioms
+    unsigned_shift_right_def val.sel(3) wityping_def wtyping_def)
+  have "property (i + 1) i tw'" and "wityping \<Gamma> (snd tw')"
+    using correctness[OF assms(1-2)] correctness_wityping[OF assms(1-2)] by auto
+  hence "lof_wline tw' OUT (i + 1) = take len (replicate amount False @ lof_wline tw' IN i)"
+    unfolding property_def by auto
+  hence "bsOUT = take len (replicate amount False @ bsIN)" (is "_ = ?rhs")
+    unfolding bsIN_def bsOUT_def by auto
+  hence "bl_to_bin bsOUT = bl_to_bin ?rhs"
+    by auto
+  also have "... = (bin_rest ^^ amount) (bl_to_bin (replicate amount False @ bsIN))"
+    using take_rest_bl2bin[where n="amount"] \<open>length bsIN = len\<close> 
+    by (metis add_diff_cancel_left' length_append length_replicate)
+  also have "... = (bin_rest ^^ amount) (bl_to_bin bsIN)"
+    using bl_to_bin_rep_F by auto
+  also have "... = bl_to_bin bsIN div 2 ^ amount"
+    unfolding bin_rest_compow by auto
+  finally have "bl_to_bin bsOUT = bl_to_bin bsIN div 2 ^ amount"
+    by auto
+  thus ?thesis
+    unfolding bl_to_bin_correctness by auto
+qed
+
+end
+
+locale signed_shift_right =
+  fixes \<Gamma> :: "sig tyenv"
+  fixes len :: nat
+  fixes amount :: nat
+  assumes "0 < len"
+  assumes "\<Gamma> IN = Lty Sig len \<and> \<Gamma> OUT = Lty Sig len"
+begin
+
+lemma well_typed:
+  "seq_wt \<Gamma> (Bassign_trans OUT (Bshiftr (Bsig IN) n) 1)"
+  by (rule seq_wt.intros(4))
+     (metis bexp_wt.intros(24) bexp_wt.intros(3) signed_shift_right_axioms signed_shift_right_def)
+
+abbreviation "lof_wline tw sig n \<equiv> lval_of (wline_of tw sig n)"
+
+text \<open>Here we factor out common expression in both inv1 and inv2. It is parametrised by the index
+we are interested with for C (first argument) and A (the second argument). Note that the index
+we are interested with for A should be the same as the index for B.\<close>
+
+definition property :: "nat \<Rightarrow> nat \<Rightarrow> sig assn2" where
+  "property idxc idx =
+      (\<lambda>tw. let bs = lof_wline tw IN idx in lof_wline tw OUT idxc = take len (replicate amount (hd bs) @ bs))"
+
+definition inv :: "sig assn2" where
+  "inv tw \<equiv> (\<forall>i < fst tw. property (i + 1) i tw)"
+
+definition inv2 :: "sig assn2" where
+  "inv2 tw \<equiv> (disjnt {IN} (event_of tw) \<longrightarrow> (\<forall>i \<ge> fst tw. property (i + 1) (fst tw) tw))"
+
+abbreviation "next_world tw \<equiv> (next_time_world tw, snd tw)"
+
+lemma inv_next_time:
+  assumes "inv tw"
+  assumes "beval_world_raw2 tw (Bshiftr (Bsig IN) amount) v" and "type_of v = Lty Sig len"
+  defines "tw' \<equiv> tw[OUT, 1 :=\<^sub>2 v]"
+  shows   "inv (next_time_world tw', snd tw')"
+  unfolding inv_def
+proof (rule, rule)
+  fix i
+  assume "i < fst (next_world tw')"
+  hence "i < next_time_world tw'"
+    by auto
+  let ?bs = "lof_wline tw IN i"
+  let ?bs' = "lof_wline tw' IN i"
+  have "fst tw' < next_time_world tw'"
+    using next_time_world_at_least  using nat_less_le by blast
+  moreover have "fst tw = fst tw'"
+    unfolding tw'_def worldline_upd2_def worldline_upd_def by auto
+  ultimately have "fst tw < next_time_world tw'"
+    by auto
+  hence "i < fst tw \<or> fst tw \<le> i \<and> i < next_time_world tw' - 1 \<or> i = next_time_world tw' - 1"
+    using \<open>i < next_time_world tw'\<close> by linarith
+  moreover
+  { assume "i < fst tw"
+    have "lof_wline tw' OUT (i + 1) = lof_wline tw OUT (i + 1)"
+      by (metis \<open>i < get_time tw\<close> add_mono1 tw'_def worldline_upd2_before_dly)
+    also have "... = take len (replicate amount (hd ?bs) @ ?bs)"
+      using assms(1) \<open>i < fst tw\<close> unfolding inv_def property_def Let_def by auto
+    also have "... = take len (replicate amount (hd ?bs') @ ?bs')"
+      by (metis \<open>i < get_time tw\<close> add.commute trans_less_add2 tw'_def worldline_upd2_before_dly)
+    finally have "property (i + 1) i (next_time_world tw', snd tw')"
+      unfolding property_def Let_def by auto }
+  moreover
+  { assume "fst tw \<le> i \<and> i < next_time_world tw' - 1"
+    hence "fst tw \<le> i" and "i < next_time_world tw' - 1"
+      by auto
+    hence "lof_wline tw' OUT (i + 1) = lof_wline tw' OUT (fst tw + 1)"
+      using unchanged_until_next_time_world
+      by (metis (mono_tags, lifting) Suc_eq_plus1 \<open>get_time tw = get_time tw'\<close> le_Suc_eq le_add1
+          le_less_trans less_diff_conv)
+    moreover have "lof_wline tw' IN i = lof_wline tw' IN (fst tw)" 
+      using unchanged_until_next_time_world
+      by (metis \<open>get_time tw = get_time tw'\<close> \<open>get_time tw \<le> i\<close> \<open>i < next_time_world tw'\<close>)
+    moreover have "property (fst tw + 1) (fst tw) tw'"
+    proof -
+      have assm2: "beval_world_raw (snd tw) (fst tw) (Bshiftr (Bsig IN) amount) v"
+        using assms(2) unfolding beval_world_raw2_def by auto
+      have "wline_of tw' OUT (fst tw + 1) = v"
+        unfolding tw'_def worldline_upd2_def worldline_upd_def by auto
+      also have "... =  Lv Sig (take len (replicate amount (hd (lof_wline tw IN (fst tw))) @ lof_wline tw IN (fst tw)))"
+        apply (rule beval_world_raw_cases[OF assm2])
+        apply ( erule_tac[!] beval_cases)+
+        prefer 2
+        unfolding state_of_world_def 
+        apply (metis (no_types, lifting) assms(3) comp_eq_dest_lhs length_append length_replicate
+               length_take min_minus min_pm take_append take_replicate ty.inject type_of.simps(2)
+               val.sel(3))
+        using assms(3) by auto
+      also have "... =  Lv Sig (take len (replicate amount (hd (lof_wline tw' IN (fst tw))) @ lof_wline tw' IN (fst tw)))"
+        by (metis less_add_one tw'_def worldline_upd2_before_dly)
+      finally show ?thesis
+        unfolding property_def bin_to_bl_def by auto
+    qed
+    ultimately have "property (i + 1) i (next_world tw')"
+      unfolding property_def by auto }
+  moreover
+  { assume "i = next_time_world tw' - 1"
+    hence "lof_wline tw' OUT (i + 1) = lof_wline tw' OUT (next_time_world tw')"
+      using \<open>i < next_time_world tw'\<close> by force
+    also have "... = lof_wline tw' OUT (fst tw + 1)"
+      using \<open>fst tw < next_time_world tw'\<close> unfolding tw'_def worldline_upd2_def
+      worldline_upd_def by auto
+    finally have "lof_wline tw' OUT (i + 1) = lof_wline tw' OUT (fst tw + 1)"
+      by auto
+    moreover have "property (fst tw + 1) (fst tw) tw'"
+    proof -
+      have assm2: "beval_world_raw (snd tw) (fst tw) (Bshiftr (Bsig IN) amount) v"
+        using assms(2) unfolding beval_world_raw2_def by auto
+      have "wline_of tw' OUT (fst tw + 1) = v"
+        unfolding tw'_def worldline_upd2_def worldline_upd_def by auto
+      also have "... =  Lv Sig (take len (replicate amount (hd (lof_wline tw IN (fst tw))) @ lof_wline tw IN (fst tw)))"
+        apply (rule beval_world_raw_cases[OF assm2])
+        apply ( erule_tac[!] beval_cases)+
+        prefer 2
+        unfolding state_of_world_def 
+        apply (metis (no_types, lifting) assms(3) comp_eq_dest_lhs length_append length_replicate
+               length_take min_minus min_pm take_append take_replicate ty.inject type_of.simps(2)
+               val.sel(3))
+        using assms(3) by auto
+      also have "... =  Lv Sig (take len (replicate amount (hd (lof_wline tw' IN (fst tw))) @ lof_wline tw' IN (fst tw)))"
+        by (metis less_add_one tw'_def worldline_upd2_before_dly)
+      finally show ?thesis
+        unfolding property_def bin_to_bl_def by auto
+    qed
+    moreover have "lof_wline tw' IN i = lof_wline tw' IN (fst tw)"
+      using unchanged_until_next_time_world
+      by (metis \<open>get_time tw < next_time_world tw'\<close> \<open>get_time tw = get_time tw'\<close> \<open>i <
+      next_time_world tw'\<close> \<open>i = next_time_world tw' - 1\<close> add_le_imp_le_diff discrete)+
+    ultimately have "property (i + 1) i (next_world tw')"
+      unfolding property_def by auto }
+  ultimately show "property (i + 1) i (next_world tw')"
+    by auto
+qed
+
+lemma type_correctness_length:
+  assumes "wityping \<Gamma> (snd tw)"
+  assumes "beval_world_raw2 tw (Bshiftr (Bsig IN) amount) v"
+  shows   "type_of v = Lty Sig len"
+proof -
+  have "beval_world_raw (snd tw) (fst tw) (Bshiftr (Bsig IN) amount) v"
+    using assms(2) unfolding beval_world_raw2_def by auto
+  have *: "type_of (state_of_world (snd tw) (fst tw) IN) = Lty Sig len"    
+    using assms(1) unfolding wityping_def
+    by (metis state_of_world_def signed_shift_right_axioms signed_shift_right_def wtyping_def)
+  show ?thesis
+    apply (rule beval_world_raw_cases[OF \<open>beval_world_raw (snd tw) (fst tw) (Bshiftr (Bsig IN) amount) v\<close>])
+    apply (erule beval_cases)+
+    unfolding state_of_world_def 
+    apply (metis "*" length_append length_replicate length_take min_minus min_pm state_of_world_def type_of.simps(2))
+    apply (erule beval_cases)+
+    apply (metis "*" length_append length_replicate length_take min_minus min_pm state_of_world_def type_of.simps(2))
+    done
+qed
+
+lemma seq_hoare_next_time:
+  "\<turnstile> [\<lambda>tw. inv tw \<and> wityping \<Gamma> (snd tw)]
+        Bassign_trans OUT (Bshiftr (Bsig IN) amount) 1
+     [\<lambda>tw. inv (next_world tw)]"
+  apply (rule Conseq2[where Q="\<lambda>tw. inv (next_world tw) \<and> wityping \<Gamma> (snd tw)", rotated 1], rule Assign2, simp)
+  using inv_next_time type_correctness_length
+  by (metis BassignE_hoare2 seq_stmt_preserve_wityping_hoare well_typed)
+
+lemma seq_hoare_next_time0:
+  "\<turnstile> [\<lambda>tw. fst tw = 0 \<and> wityping \<Gamma> (snd tw)]
+        Bassign_trans OUT (Bshiftr (Bsig IN) amount) 1
+     [\<lambda>tw. inv (next_world tw)]"
+  apply (rule Conseq2[where Q="\<lambda>tw. inv (next_world tw) \<and> wityping \<Gamma> (snd tw)", rotated 1], rule Assign2, simp)
+  using inv_next_time type_correctness_length unfolding inv_def
+  by (metis BassignE_hoare2 gr_implies_not_zero seq_stmt_preserve_wityping_hoare well_typed)
+
+lemma conc_hoare:
+  "\<And>tw. inv tw \<and> inv2 tw \<and> disjnt {IN} (event_of tw) \<Longrightarrow> inv (next_world tw)"
+proof -
+  fix tw
+  assume "inv tw \<and> inv2 tw \<and> disjnt {IN} (event_of tw)"
+  hence "inv tw" and "inv2 tw" and "disjnt {IN} (event_of tw)"
+    by auto
+  { fix i
+    assume "i < next_time_world tw"
+    have "fst tw < next_time_world tw"
+      by (simp add: next_time_world_at_least)
+    have "i < fst tw \<or> fst tw \<le> i"
+      by auto
+    moreover
+    { assume "i < fst tw"
+      hence "property (i + 1) i tw"
+        using \<open>inv tw\<close> unfolding inv_def by auto
+      hence "property (i + 1) i (next_world tw)"
+        unfolding property_def by simp }
+    moreover
+    { assume "fst tw \<le> i"
+      moreover have "\<forall>i \<ge> fst tw. property (i + 1) (fst tw) tw"
+        using \<open>inv2 tw\<close> \<open>disjnt {IN} (event_of tw)\<close> unfolding inv2_def
+        by auto
+      ultimately have "property (i + 1) (fst tw) tw"
+        by auto
+      hence "property (i + 1) i tw"
+        unfolding property_def
+        by (metis \<open>get_time tw \<le> i\<close> \<open>i < next_time_world tw\<close> unchanged_until_next_time_world)
+      hence "property (i + 1) i (next_world tw)"
+        unfolding property_def by auto }
+    ultimately have "property (i + 1) i (next_world tw)"
+      by auto }
+  thus "inv (next_world tw)"
+    unfolding inv_def by auto
+qed
+
+lemma conc_hoare2:
+  "\<And>tw. inv tw \<and> inv2 tw \<and> disjnt {IN} (event_of tw) \<Longrightarrow> inv2 (next_world tw)"
+proof -
+  fix tw
+  assume "inv tw \<and> inv2 tw \<and> disjnt {IN} (event_of tw)"
+  hence "inv tw" and "inv2 tw" and "disjnt {IN} (event_of tw)"
+    by auto
+  let ?t' = "next_time_world tw"
+  { assume "disjnt {IN} (event_of (next_world tw))"
+    hence *: "lof_wline tw IN ?t' = lof_wline tw IN (?t' - 1)"
+      unfolding event_of_alt_def
+      by (smt comp_apply diff_0_eq_0 disjnt_insert1 fst_conv mem_Collect_eq snd_conv)
+    have "fst tw < ?t'"
+      by (simp add: next_time_world_at_least)
+    { fix i
+      assume "?t' \<le> i"
+      have "property (i + 1) (fst tw) tw"
+        using \<open>inv2 tw\<close> \<open>disjnt {IN} (event_of tw)\<close> unfolding inv2_def
+        using \<open>get_time tw < next_time_world tw\<close> \<open>next_time_world tw \<le> i\<close> by auto
+      moreover have "lof_wline tw IN (fst tw) = lof_wline tw IN (?t' - 1)"
+        by (metis \<open>get_time tw < next_time_world tw\<close> add_le_imp_le_diff diff_less discrete
+        gr_implies_not0 not_less_iff_gr_or_eq unchanged_until_next_time_world zero_less_one)
+      ultimately have "property (i + 1) ?t' (next_world tw)"
+        unfolding property_def using *  by auto }
+    hence "\<forall>i\<ge>?t'. property (i + 1) ?t' (next_world tw)"
+      by auto }
+  thus "inv2 (next_world tw)"
+    unfolding inv2_def by auto
+qed
+
+lemma inv2_next_time:
+  fixes tw
+  assumes "beval_world_raw2 tw (Bshiftr (Bsig IN) amount) v" and "type_of v = Lty Sig len"
+  defines "tw' \<equiv> tw[OUT, 1 :=\<^sub>2 v]"
+  shows   "inv2 (next_time_world tw', snd tw')"
+  unfolding inv2_def
+proof (rule, rule, rule)
+  fix i
+  assume "disjnt {IN} (event_of (next_world tw'))"
+  hence "IN \<notin> event_of (next_world tw')"
+    by auto
+  assume "fst (next_world tw') \<le> i"
+  hence "next_time_world tw' \<le> i"
+    by auto
+  let ?t' = "next_time_world tw'"
+  have "fst tw' < ?t'"
+    using next_time_world_at_least by blast
+  moreover have "fst tw = fst tw'"
+    unfolding tw'_def unfolding worldline_upd2_def by auto
+  ultimately have "fst tw < ?t'"
+    by auto
+  have 0: "wline_of (next_world tw') IN ?t' = wline_of tw IN (fst tw)"
+  proof -
+    have "wline_of tw' IN ?t' = wline_of tw' IN (?t' - 1)"
+      using \<open>IN \<notin> event_of (next_world tw')\<close> unfolding event_of_alt_def
+      using \<open>get_time tw' < next_time_world tw'\<close> by auto
+    also have " ... = wline_of tw' IN (fst tw')"
+      using unchanged_until_next_time_world
+      by (metis (no_types, lifting) Suc_diff_1 \<open>get_time tw' < next_time_world tw'\<close> diff_less
+      gr_implies_not_zero le_0_eq less_Suc_eq_le not_less zero_less_one)
+    also have "... = wline_of tw' IN (fst tw)"
+      by (simp add: \<open>get_time tw = get_time tw'\<close>)
+    also have "... = wline_of tw IN (fst tw)"
+      unfolding tw'_def worldline_upd2_def worldline_upd_def by auto
+    finally show "wline_of (next_world tw') IN ?t' = wline_of tw IN (fst tw)"
+      by auto
+  qed
+  have assm2: "beval_world_raw (snd tw) (fst tw) (Bshiftr (Bsig IN) amount) v"
+    using assms(1) unfolding beval_world_raw2_def by auto
+  have "wline_of (next_world tw') OUT (i + 1) = v"
+  proof -
+    have "wline_of tw' OUT (i + 1) = v"
+      using `fst tw < ?t'` \<open>?t' \<le> i\<close>
+      unfolding tw'_def worldline_upd2_def worldline_upd_def by auto
+    thus ?thesis
+      by auto
+  qed
+  also have "lval_of ... = take len (replicate amount (hd (lof_wline tw IN (fst tw))) @ lof_wline tw IN (fst tw))"
+    apply (rule beval_world_raw_cases[OF assm2])
+    apply (erule_tac[!] beval_cases)+
+    prefer 2
+    apply (metis (no_types, lifting) assms(2) comp_def length_append length_replicate length_take min_minus min_pm state_of_world_def take_append take_replicate ty.inject type_of.simps(2) val.sel(3))
+    using assms(2) by auto
+  finally have "property (i + 1) ?t' (next_world tw')"
+    unfolding property_def using 0  by auto
+  thus "property (i + 1) (get_time (next_time_world tw', snd tw')) (next_time_world tw', snd tw')"
+    by auto
+qed
+
+lemma seq_hoare_next_time1:
+  shows "\<turnstile> [\<lambda>tw. wityping \<Gamma> (snd tw)] Bassign_trans OUT (Bshiftr (Bsig IN) amount) 1 [\<lambda>tw. inv2 (next_time_world tw, snd tw)]"
+  apply (rule Assign2_altI)
+  using inv2_next_time  type_correctness_length by blast
+
+lemma conc_hoare3:
+  "\<turnstile> \<lbrace>\<lambda>tw. (inv tw \<and> wityping \<Gamma> (snd tw)) \<and> inv2 tw\<rbrace> shiftr amount \<lbrace>\<lambda>tw. inv (next_time_world tw, snd tw) \<and> inv2 (next_time_world tw, snd tw)\<rbrace>"
+  unfolding shiftr_def
+  apply (rule Single)
+   apply (rule Conj)
+    apply (rule strengthen_precondition)
+  apply (rule strengthen_precondition)
+    apply (rule seq_hoare_next_time)
+  apply (rule strengthen_precondition)
+   apply (rule strengthen_precondition)
+   apply (rule strengthen_precondition2)
+   apply (rule seq_hoare_next_time1)
+  using conc_hoare conc_hoare2 by blast
+
+lemma seq_wt_sub:
+  "seq_wt \<Gamma> (Bassign_trans OUT (Bshiftr (Bsig IN) amount) 1)"
+  using well_typed by blast
+
+lemma conc_hoare4:
+  "\<turnstile> \<lbrace>\<lambda>tw. (inv tw \<and> wityping \<Gamma> (snd tw)) \<and> inv2 tw\<rbrace> shiftr amount \<lbrace>\<lambda>tw. (inv (next_time_world tw, snd tw) \<and> wityping \<Gamma> (snd tw)) \<and> inv2 (next_time_world tw, snd tw)\<rbrace>"
+  apply (rule Conj2)
+   apply (rule Conj2)
+    apply (rule weaken_post_conc_hoare[OF _ conc_hoare3], blast)
+   apply (rule strengthen_pre_conc_hoare[rotated])
+    apply (unfold shiftr_def, rule single_conc_stmt_preserve_wityping_hoare)
+    apply (rule seq_wt_sub)
+   apply blast
+  apply (fold shiftr_def, rule weaken_post_conc_hoare[OF _ conc_hoare3], blast)
+  done
+
+lemma conc_sim':
+  "\<turnstile>\<^sub>s \<lbrace>\<lambda>tw. (inv tw \<and> wityping \<Gamma> (snd tw)) \<and> inv2 tw\<rbrace> shiftr amount \<lbrace>\<lambda>tw. (inv tw \<and> wityping \<Gamma> (snd tw)) \<and> inv2 tw\<rbrace>"
+  apply (rule While)
+  apply (unfold snd_conv, rule conc_hoare4)
+  done
+
+lemma conc_sim2:
+  "\<turnstile>\<^sub>s \<lbrace>\<lambda>tw. (inv tw \<and> wityping \<Gamma> (snd tw)) \<and> inv2 tw\<rbrace> shiftr amount \<lbrace>inv\<rbrace>"
+  using conc_sim' Conseq_sim by blast
+
+lemma init_sat_inv:
+  "init_sim_hoare (\<lambda>tw. fst tw = 0 \<and> wityping \<Gamma> (snd tw)) (shiftr amount) (\<lambda>tw. inv tw \<and> wityping \<Gamma> (snd tw))"
+  unfolding shiftr_def
+  apply (rule AssignI)
+  apply (rule SingleI)
+  apply (rule Conj)
+  unfolding snd_conv apply(rule seq_hoare_next_time0)
+  apply (rule strengthen_precondition2)
+  by (metis seq_stmt_preserve_wityping_hoare well_typed)
+
+lemma init_sat_inv2:
+  "init_sim_hoare (\<lambda>tw. wityping \<Gamma> (snd tw)) (shiftr amount) inv2"
+  unfolding shiftr_def
+  apply (rule AssignI)
+  apply (rule SingleI)
+  unfolding snd_conv apply (rule seq_hoare_next_time1)
+  done
+
+lemma init_sat_inv_comb:
+  shows "init_sim_hoare (\<lambda>tw. fst tw = 0 \<and> wityping \<Gamma> (snd tw)) (shiftr amount)  (\<lambda>tw. (inv tw \<and> wityping \<Gamma> (snd tw)) \<and> inv2 tw)"
+  apply (rule ConjI_sim)
+  apply (rule init_sat_inv)
+  apply (rule ConseqI_sim[rotated])
+  apply (rule init_sat_inv2)
+  by blast+
+
+lemma correctness:
+  assumes "sim_fin w (i + 1) (shiftr amount) tw'" and "wityping \<Gamma> w"
+  shows   "property (i + 1) i tw'"
+proof -
+  obtain tw where "init_sim (0, w) (shiftr amount) tw" and  "tw, i + 1, shiftr amount \<Rightarrow>\<^sub>S tw'"
+    using premises_sim_fin_obt[OF assms(1)] by auto
+  hence "i + 1 < fst tw'"
+    using world_maxtime_lt_fst_tres  by blast
+  have "conc_stmt_wf (shiftr amount)"
+    unfolding conc_stmt_wf_def shiftr_def by auto
+  moreover have "nonneg_delay_conc (shiftr amount)"
+    unfolding shiftr_def by auto
+  ultimately have "init_sim_valid (\<lambda>tw. fst tw = 0 \<and> wityping \<Gamma> (snd tw)) (shiftr amount) (\<lambda>tw. (inv tw \<and> wityping \<Gamma> (snd tw)) \<and> inv2 tw)"
+    using init_sim_hoare_soundness[OF init_sat_inv_comb]
+    by (metis (no_types, lifting) conc_wt_cases(1) init_sat_inv_comb
+    init_sim_hoare_soundness sub_def strengthen_precondition_init_sim_hoare)
+  hence "inv tw \<and> wityping \<Gamma> (snd tw) \<and> inv2 tw"
+    using \<open>init_sim (0, w) (shiftr amount) tw\<close> fst_conv assms(2) unfolding init_sim_valid_def
+    by (metis snd_conv)
+  hence "inv tw" and "inv2 tw" and "wityping \<Gamma> (snd tw)"
+    by auto
+  moreover have "\<Turnstile>\<^sub>s \<lbrace>\<lambda>tw. (inv tw \<and> wityping \<Gamma> (snd tw)) \<and> inv2 tw\<rbrace> shiftr amount \<lbrace>inv\<rbrace>"
+    using conc_sim_soundness[OF conc_sim2] \<open>conc_stmt_wf (shiftr amount)\<close> \<open>nonneg_delay_conc (shiftr amount)\<close>
+    by auto
+  ultimately have "inv tw'"
+    using \<open>tw, i + 1, shiftr amount \<Rightarrow>\<^sub>S tw'\<close> unfolding sim_hoare_valid_def by blast
+  with \<open>i + 1 < fst tw'\<close> show ?thesis
+    unfolding inv_def by auto
+qed
+
+lemma correctness_wityping:
+  assumes "sim_fin w (i + 1) (shiftr amount) tw'" and "wityping \<Gamma> w"
+  shows   "wityping \<Gamma> (snd tw')"
+proof -
+  obtain tw where "init_sim (0, w) (shiftr amount) tw" and  "tw, i + 1, (shiftr amount) \<Rightarrow>\<^sub>S tw'"
+    using premises_sim_fin_obt[OF assms(1)] by auto
+  hence "i + 1 < fst tw'"
+    using world_maxtime_lt_fst_tres  by blast
+  have "conc_stmt_wf (shiftr amount)"
+    unfolding conc_stmt_wf_def shiftr_def by auto
+  moreover have "nonneg_delay_conc (shiftr amount)"
+    unfolding shiftr_def by auto
+  ultimately have "init_sim_valid (\<lambda>tw. fst tw = 0 \<and> wityping \<Gamma> (snd tw)) (shiftr amount) (\<lambda>tw. (inv tw \<and> wityping \<Gamma> (snd tw)) \<and> inv2 tw)"
+    using init_sim_hoare_soundness[OF init_sat_inv_comb]
+    by (metis (no_types, lifting) conc_wt_cases(1) init_sat_inv_comb
+    init_sim_hoare_soundness sub_def strengthen_precondition_init_sim_hoare)
+  hence "inv tw \<and> wityping \<Gamma> (snd tw) \<and> inv2 tw"
+    using \<open>init_sim (0, w) (shiftr amount) tw\<close> fst_conv assms(2) unfolding init_sim_valid_def
+    by (metis snd_conv)
+  hence "inv tw" and "inv2 tw" and "wityping \<Gamma> (snd tw)"
+    by auto
+  moreover have "\<Turnstile>\<^sub>s \<lbrace>\<lambda>tw. (inv tw \<and> wityping \<Gamma> (snd tw)) \<and> inv2 tw\<rbrace> (shiftr amount) \<lbrace>\<lambda>tw. wityping \<Gamma> (snd tw)\<rbrace>"
+    using conc_sim_soundness[OF conc_sim'] \<open>conc_stmt_wf (shiftr amount)\<close> \<open>nonneg_delay_conc (shiftr amount)\<close>
+    by (smt sim_hoare_valid_def)  
+  ultimately show "wityping \<Gamma> (snd tw')"
+    using \<open>tw, i + 1, (shiftr amount) \<Rightarrow>\<^sub>S tw'\<close> unfolding sim_hoare_valid_def by blast
+qed
+
+corollary correctness2:
+  assumes "sim_fin w (i + 1) (shiftr amount) tw'" and "wityping \<Gamma> w"
+  defines "bsIN  \<equiv> lof_wline tw' IN i"
+  defines "bsOUT \<equiv> lof_wline tw' OUT (i + 1)"
+  shows   "sbl_to_bin bsOUT = sbl_to_bin bsIN div 2 ^ amount" and "length bsIN = len" and "length bsOUT = len"
+proof -
+  have "wityping \<Gamma> (snd tw')"
+    using correctness_wityping[OF assms(1-2)] by auto
+  thus "length bsIN = len"
+    by (smt assms(3) o_apply ty.distinct(1) ty.inject type_of.elims signed_shift_right_axioms
+        signed_shift_right_def val.sel(3) wityping_def wtyping_def)
+  have "property (i + 1) i tw'" and "wityping \<Gamma> (snd tw')"
+    using correctness[OF assms(1-2)] correctness_wityping[OF assms(1-2)] by auto
+  hence "lof_wline tw' OUT (i + 1) = take len (replicate amount (hd (lof_wline tw' IN i)) @ lof_wline tw' IN i)"
+    unfolding property_def Let_def by auto
+  hence "bsOUT = take len (replicate amount (hd (bsIN)) @ bsIN)" (is "_ = ?rhs")
+    unfolding bsIN_def bsOUT_def by auto
+  hence "sbl_to_bin bsOUT = sbl_to_bin ?rhs"
+    by auto
+  also have "... = (bin_rest ^^ amount) (sbl_to_bin (replicate amount (hd bsIN) @ bsIN))"
+    using take_rest_sbl2bin[where n="amount" and bl="replicate amount (hd bsIN) @ bsIN"] \<open>length bsIN = len\<close> 
+    signed_shift_right_axioms signed_shift_right_def by simp
+  also have "... = (bin_rest ^^ amount) (sbl_to_bin bsIN)"
+    using sbl_to_bin_replicate_app \<open>length bsIN = len\<close> signed_shift_right_axioms
+    signed_shift_right_def by auto
+  also have "... = sbl_to_bin bsIN div 2 ^ amount"
+    unfolding bin_rest_compow by auto
+  finally show "sbl_to_bin bsOUT = sbl_to_bin bsIN div 2 ^ amount"
+    by auto
+  show "length bsOUT = len"
+    using \<open>bsOUT = take len (replicate amount (hd (bsIN)) @ bsIN)\<close> 
+    by (simp add: \<open>length bsIN = len\<close>)
+qed
+
+corollary correctness3:
+  assumes "sim_fin w (i + 1) (shiftr amount) tw'" and "wityping \<Gamma> w"
+  defines "bsIN  \<equiv> lof_wline tw' IN i"
+  defines "bsOUT \<equiv> lof_wline tw' OUT (i + 1)"
+  shows   "- (int \<circ> of_bool) (hd bsOUT) * 2 ^ (len - 1) + (\<Sum>i = 0..<len - 1. (int \<circ> of_bool) (rev (tl bsOUT) ! i) * 2 ^ i) =
+          (- (int \<circ> of_bool) (hd bsIN ) * 2 ^ (len - 1) + (\<Sum>i = 0..<len - 1. (int \<circ> of_bool) (rev (tl bsIN ) ! i) * 2 ^ i)) div 2 ^ amount"
+proof -
+  have 0: "sbl_to_bin bsOUT = sbl_to_bin bsIN div 2 ^ amount" and "length bsIN = len" and "length bsOUT = len"
+    using correctness2 assms by auto
+  have 1: "bsIN = hd bsIN # tl bsIN"
+    using \<open>length bsIN = len\<close> list.exhaust_sel signed_shift_right_axioms signed_shift_right_def by auto
+  have 2: "bsOUT = hd bsOUT # tl bsOUT"
+    using \<open>length bsOUT = len\<close> signed_shift_right_axioms signed_shift_right_def by auto
+  hence 3: "sbl_to_bin bsOUT = - (int \<circ> of_bool) (hd bsOUT) * 2 ^ (len - 1) + (\<Sum>i = 0..<len - 1. (int \<circ> of_bool) (rev (tl bsOUT) ! i) * 2 ^ i)"
+    using sbl_to_bin_correctness 
+    by (metis (no_types, lifting) \<open>length bsOUT = len\<close> length_tl sum.cong)
+  have 4: "sbl_to_bin bsIN = - (int \<circ> of_bool) (hd bsIN ) * 2 ^ (len - 1) + (\<Sum>i = 0..<len-1. (int \<circ> of_bool) (rev (tl bsIN ) ! i) * 2 ^ i)"
+    using sbl_to_bin_correctness 
+    by (metis (full_types) "1" \<open>length bsIN = len\<close> length_tl)
+  show ?thesis
+    using 0 unfolding 3 4 by auto
+qed
+
+end
+
+end
+
